QCP_examples/humaneval/spec_logic_rewrite_c_files/C_161_goal.v
@@ -1,0 +1,1831 @@
+Require Import Coq.ZArith.ZArith.
+Require Import Coq.Bool.Bool.
+Require Import Coq.Strings.String.
+Require Import Coq.Strings.Ascii.
+Require Import Coq.Lists.List.
+Require Import Coq.Classes.RelationClasses.
+Require Import Coq.Classes.Morphisms.
+Require Import Coq.micromega.Psatz.
+Require Import Coq.Sorting.Permutation.
+From AUXLib Require Import int_auto Axioms Feq Idents ListLib VMap.
+Require Import SetsClass.SetsClass. Import SetsNotation.
+From SimpleC.SL Require Import Mem SeparationLogic.
+Require Import Logic.LogicGenerator.demo932.Interface.
+Local Open Scope Z_scope.
+Local Open Scope sets.
+Local Open Scope string_scope.
+Local Open Scope list.
+Import naive_C_Rules.
+Require Import SimpleC.StdLib.string_lib.
+Require Import coins_161.
+Local Open Scope sac.
+From SimpleC.EE.QCP_demos_LLM Require Import char_array_strategy_goal.
+From SimpleC.EE.QCP_demos_LLM Require Import char_array_strategy_proof.
+From SimpleC.StdLib Require Import string_strategy_goal.
+From SimpleC.StdLib Require Import string_strategy_proof.
+
+(*----- Function solve -----*)
+
+Definition solve_safety_wit_1 := 
+forall (s_pre: Z) (input: (@list Z)) (retval: Z) (PreH1 : (retval = (string_length (input)))) (PreH2 : (0 <= ((string_length (input)) + 1 ))) (PreH3 : (valid_string input )) (PreH4 : (problem_161_pre_z input )) (PreH5 : (ascii_range_z input )) (PreH6 : ((string_length (input)) < INT_MAX)) ,
+  ((( &( "nletter" ) )) # Int  |->_)
+  **  (store_string s_pre input )
+  **  ((( &( "n" ) )) # Int  |-> retval)
+  **  ((( &( "s" ) )) # Ptr  |-> s_pre)
+|--
+  “ (0 <= INT_MAX) ” 
+  &&  “ ((INT_MIN) <= 0) ”
+.
+
+Definition solve_safety_wit_2 := 
+forall (s_pre: Z) (input: (@list Z)) (retval: Z) (PreH1 : (retval = (string_length (input)))) (PreH2 : (0 <= ((string_length (input)) + 1 ))) (PreH3 : (valid_string input )) (PreH4 : (problem_161_pre_z input )) (PreH5 : (ascii_range_z input )) (PreH6 : ((string_length (input)) < INT_MAX)) ,
+  ((( &( "out" ) )) # Ptr  |->_)
+  **  ((( &( "nletter" ) )) # Int  |-> 0)
+  **  (store_string s_pre input )
+  **  ((( &( "n" ) )) # Int  |-> retval)
+  **  ((( &( "s" ) )) # Ptr  |-> s_pre)
+|--
+  “ ((retval + 1 ) <= INT_MAX) ” 
+  &&  “ ((INT_MIN) <= (retval + 1 )) ”
+.
+
+Definition solve_safety_wit_3 := 
+forall (s_pre: Z) (input: (@list Z)) (retval: Z) (PreH1 : (retval = (string_length (input)))) (PreH2 : (0 <= ((string_length (input)) + 1 ))) (PreH3 : (valid_string input )) (PreH4 : (problem_161_pre_z input )) (PreH5 : (ascii_range_z input )) (PreH6 : ((string_length (input)) < INT_MAX)) ,
+  ((( &( "out" ) )) # Ptr  |->_)
+  **  ((( &( "nletter" ) )) # Int  |-> 0)
+  **  (store_string s_pre input )
+  **  ((( &( "n" ) )) # Int  |-> retval)
+  **  ((( &( "s" ) )) # Ptr  |-> s_pre)
+|--
+  “ (1 <= INT_MAX) ” 
+  &&  “ ((INT_MIN) <= 1) ”
+.
+
+Definition solve_safety_wit_4 := 
+forall (s_pre: Z) (input: (@list Z)) (retval: Z) (retval_2: Z) (PreH1 : (retval_2 <> 0)) (PreH2 : (retval = (string_length (input)))) (PreH3 : (0 <= ((string_length (input)) + 1 ))) (PreH4 : (valid_string input )) (PreH5 : (problem_161_pre_z input )) (PreH6 : (ascii_range_z input )) (PreH7 : ((string_length (input)) < INT_MAX)) ,
+  (CharArray.undef_full retval_2 (retval + 1 ) )
+  **  (CharArray.full s_pre ((string_length (input)) + 1 ) (c_string (input)) )
+  **  ((( &( "out" ) )) # Ptr  |-> retval_2)
+  **  ((( &( "nletter" ) )) # Int  |-> 0)
+  **  ((( &( "n" ) )) # Int  |-> retval)
+  **  ((( &( "s" ) )) # Ptr  |-> s_pre)
+|--
+  “ (0 <= INT_MAX) ” 
+  &&  “ ((INT_MIN) <= 0) ”
+.
+
+Definition solve_safety_wit_5 := 
+forall (s_pre: Z) (input: (@list Z)) (retval: Z) (retval_2: Z) (PreH1 : (retval_2 = 0)) (PreH2 : (retval_2 <> 0)) (PreH3 : (retval = (string_length (input)))) (PreH4 : (0 <= ((string_length (input)) + 1 ))) (PreH5 : (valid_string input )) (PreH6 : (problem_161_pre_z input )) (PreH7 : (ascii_range_z input )) (PreH8 : ((string_length (input)) < INT_MAX)) ,
+  (CharArray.undef_full retval_2 (retval + 1 ) )
+  **  (CharArray.full s_pre ((string_length (input)) + 1 ) (c_string (input)) )
+  **  ((( &( "out" ) )) # Ptr  |-> retval_2)
+  **  ((( &( "nletter" ) )) # Int  |-> 0)
+  **  ((( &( "n" ) )) # Int  |-> retval)
+  **  ((( &( "s" ) )) # Ptr  |-> s_pre)
+|--
+  “ False ”
+.
+
+Definition solve_safety_wit_6 := 
+forall (s_pre: Z) (input: (@list Z)) (retval: Z) (retval_2: Z) (PreH1 : (retval_2 <> 0)) (PreH2 : (retval_2 <> 0)) (PreH3 : (retval = (string_length (input)))) (PreH4 : (0 <= ((string_length (input)) + 1 ))) (PreH5 : (valid_string input )) (PreH6 : (problem_161_pre_z input )) (PreH7 : (ascii_range_z input )) (PreH8 : ((string_length (input)) < INT_MAX)) ,
+  ((( &( "w" ) )) # Int  |->_)
+  **  ((( &( "i" ) )) # Int  |->_)
+  **  (CharArray.undef_full retval_2 (retval + 1 ) )
+  **  (CharArray.full s_pre ((string_length (input)) + 1 ) (c_string (input)) )
+  **  ((( &( "out" ) )) # Ptr  |-> retval_2)
+  **  ((( &( "nletter" ) )) # Int  |-> 0)
+  **  ((( &( "n" ) )) # Int  |-> retval)
+  **  ((( &( "s" ) )) # Ptr  |-> s_pre)
+|--
+  “ (0 <= INT_MAX) ” 
+  &&  “ ((INT_MIN) <= 0) ”
+.
+
+Definition solve_safety_wit_7 := 
+forall (s_pre: Z) (input: (@list Z)) (retval: Z) (retval_2: Z) (PreH1 : (retval_2 <> 0)) (PreH2 : (retval_2 <> 0)) (PreH3 : (retval = (string_length (input)))) (PreH4 : (0 <= ((string_length (input)) + 1 ))) (PreH5 : (valid_string input )) (PreH6 : (problem_161_pre_z input )) (PreH7 : (ascii_range_z input )) (PreH8 : ((string_length (input)) < INT_MAX)) ,
+  ((( &( "w" ) )) # Int  |-> 0)
+  **  ((( &( "i" ) )) # Int  |->_)
+  **  (CharArray.undef_full retval_2 (retval + 1 ) )
+  **  (CharArray.full s_pre ((string_length (input)) + 1 ) (c_string (input)) )
+  **  ((( &( "out" ) )) # Ptr  |-> retval_2)
+  **  ((( &( "nletter" ) )) # Int  |-> 0)
+  **  ((( &( "n" ) )) # Int  |-> retval)
+  **  ((( &( "s" ) )) # Ptr  |-> s_pre)
+|--
+  “ (0 <= INT_MAX) ” 
+  &&  “ ((INT_MIN) <= 0) ”
+.
+
+Definition solve_safety_wit_8 := 
+forall (s_pre: Z) (input: (@list Z)) (output: (@list Z)) (w: Z) (nletter: Z) (i: Z) (out: Z) (n: Z) (PreH1 : (i < n)) (PreH2 : (n = (string_length (input)))) (PreH3 : (out <> 0)) (PreH4 : (0 <= i)) (PreH5 : (i <= n)) (PreH6 : (0 <= nletter)) (PreH7 : (nletter <= i)) (PreH8 : (0 <= w)) (PreH9 : (w <= 127)) (PreH10 : (flip_scan_state_z_161 input output i nletter )) (PreH11 : (valid_string input )) (PreH12 : (problem_161_pre_z input )) (PreH13 : (ascii_range_z input )) (PreH14 : ((string_length (input)) < INT_MAX)) ,
+  ((( &( "s" ) )) # Ptr  |-> s_pre)
+  **  ((( &( "n" ) )) # Int  |-> n)
+  **  ((( &( "out" ) )) # Ptr  |-> out)
+  **  ((( &( "i" ) )) # Int  |-> i)
+  **  ((( &( "nletter" ) )) # Int  |-> nletter)
+  **  ((( &( "w" ) )) # Int  |-> (Znth i (c_string (input)) 0))
+  **  (store_string s_pre input )
+  **  (CharArray.full out i output )
+  **  (CharArray.undef_seg out i (n + 1 ) )
+|--
+  “ (65 <= INT_MAX) ” 
+  &&  “ ((INT_MIN) <= 65) ”
+.
+
+Definition solve_safety_wit_9 := 
+forall (s_pre: Z) (input: (@list Z)) (output: (@list Z)) (w: Z) (nletter: Z) (i: Z) (out: Z) (n: Z) (PreH1 : ((Znth i (c_string (input)) 0) >= 65)) (PreH2 : (i < n)) (PreH3 : (n = (string_length (input)))) (PreH4 : (out <> 0)) (PreH5 : (0 <= i)) (PreH6 : (i <= n)) (PreH7 : (0 <= nletter)) (PreH8 : (nletter <= i)) (PreH9 : (0 <= w)) (PreH10 : (w <= 127)) (PreH11 : (flip_scan_state_z_161 input output i nletter )) (PreH12 : (valid_string input )) (PreH13 : (problem_161_pre_z input )) (PreH14 : (ascii_range_z input )) (PreH15 : ((string_length (input)) < INT_MAX)) ,
+  ((( &( "s" ) )) # Ptr  |-> s_pre)
+  **  ((( &( "n" ) )) # Int  |-> n)
+  **  ((( &( "out" ) )) # Ptr  |-> out)
+  **  ((( &( "i" ) )) # Int  |-> i)
+  **  ((( &( "nletter" ) )) # Int  |-> nletter)
+  **  ((( &( "w" ) )) # Int  |-> (Znth i (c_string (input)) 0))
+  **  (store_string s_pre input )
+  **  (CharArray.full out i output )
+  **  (CharArray.undef_seg out i (n + 1 ) )
+|--
+  “ (90 <= INT_MAX) ” 
+  &&  “ ((INT_MIN) <= 90) ”
+.
+
+Definition solve_safety_wit_10 := 
+forall (s_pre: Z) (input: (@list Z)) (output: (@list Z)) (w: Z) (nletter: Z) (i: Z) (out: Z) (n: Z) (PreH1 : ((Znth i (c_string (input)) 0) <= 90)) (PreH2 : ((Znth i (c_string (input)) 0) >= 65)) (PreH3 : (i < n)) (PreH4 : (n = (string_length (input)))) (PreH5 : (out <> 0)) (PreH6 : (0 <= i)) (PreH7 : (i <= n)) (PreH8 : (0 <= nletter)) (PreH9 : (nletter <= i)) (PreH10 : (0 <= w)) (PreH11 : (w <= 127)) (PreH12 : (flip_scan_state_z_161 input output i nletter )) (PreH13 : (valid_string input )) (PreH14 : (problem_161_pre_z input )) (PreH15 : (ascii_range_z input )) (PreH16 : ((string_length (input)) < INT_MAX)) ,
+  ((( &( "s" ) )) # Ptr  |-> s_pre)
+  **  ((( &( "n" ) )) # Int  |-> n)
+  **  ((( &( "out" ) )) # Ptr  |-> out)
+  **  ((( &( "i" ) )) # Int  |-> i)
+  **  ((( &( "nletter" ) )) # Int  |-> nletter)
+  **  ((( &( "w" ) )) # Int  |-> (Znth i (c_string (input)) 0))
+  **  (store_string s_pre input )
+  **  (CharArray.full out i output )
+  **  (CharArray.undef_seg out i (n + 1 ) )
+|--
+  “ (((Znth i (c_string (input)) 0) + 32 ) <= INT_MAX) ” 
+  &&  “ ((INT_MIN) <= ((Znth i (c_string (input)) 0) + 32 )) ”
+.
+
+Definition solve_safety_wit_11 := 
+forall (s_pre: Z) (input: (@list Z)) (output: (@list Z)) (w: Z) (nletter: Z) (i: Z) (out: Z) (n: Z) (PreH1 : ((Znth i (c_string (input)) 0) <= 90)) (PreH2 : ((Znth i (c_string (input)) 0) >= 65)) (PreH3 : (i < n)) (PreH4 : (n = (string_length (input)))) (PreH5 : (out <> 0)) (PreH6 : (0 <= i)) (PreH7 : (i <= n)) (PreH8 : (0 <= nletter)) (PreH9 : (nletter <= i)) (PreH10 : (0 <= w)) (PreH11 : (w <= 127)) (PreH12 : (flip_scan_state_z_161 input output i nletter )) (PreH13 : (valid_string input )) (PreH14 : (problem_161_pre_z input )) (PreH15 : (ascii_range_z input )) (PreH16 : ((string_length (input)) < INT_MAX)) ,
+  ((( &( "s" ) )) # Ptr  |-> s_pre)
+  **  ((( &( "n" ) )) # Int  |-> n)
+  **  ((( &( "out" ) )) # Ptr  |-> out)
+  **  ((( &( "i" ) )) # Int  |-> i)
+  **  ((( &( "nletter" ) )) # Int  |-> nletter)
+  **  ((( &( "w" ) )) # Int  |-> (Znth i (c_string (input)) 0))
+  **  (store_string s_pre input )
+  **  (CharArray.full out i output )
+  **  (CharArray.undef_seg out i (n + 1 ) )
+|--
+  “ (32 <= INT_MAX) ” 
+  &&  “ ((INT_MIN) <= 32) ”
+.
+
+Definition solve_safety_wit_12 := 
+forall (s_pre: Z) (input: (@list Z)) (output: (@list Z)) (w: Z) (nletter: Z) (i: Z) (out: Z) (n: Z) (PreH1 : ((Znth i (c_string (input)) 0) < 65)) (PreH2 : (i < n)) (PreH3 : (n = (string_length (input)))) (PreH4 : (out <> 0)) (PreH5 : (0 <= i)) (PreH6 : (i <= n)) (PreH7 : (0 <= nletter)) (PreH8 : (nletter <= i)) (PreH9 : (0 <= w)) (PreH10 : (w <= 127)) (PreH11 : (flip_scan_state_z_161 input output i nletter )) (PreH12 : (valid_string input )) (PreH13 : (problem_161_pre_z input )) (PreH14 : (ascii_range_z input )) (PreH15 : ((string_length (input)) < INT_MAX)) ,
+  ((( &( "s" ) )) # Ptr  |-> s_pre)
+  **  ((( &( "n" ) )) # Int  |-> n)
+  **  ((( &( "out" ) )) # Ptr  |-> out)
+  **  ((( &( "i" ) )) # Int  |-> i)
+  **  ((( &( "nletter" ) )) # Int  |-> nletter)
+  **  ((( &( "w" ) )) # Int  |-> (Znth i (c_string (input)) 0))
+  **  (store_string s_pre input )
+  **  (CharArray.full out i output )
+  **  (CharArray.undef_seg out i (n + 1 ) )
+|--
+  “ (97 <= INT_MAX) ” 
+  &&  “ ((INT_MIN) <= 97) ”
+.
+
+Definition solve_safety_wit_13 := 
+forall (s_pre: Z) (input: (@list Z)) (output: (@list Z)) (w: Z) (nletter: Z) (i: Z) (out: Z) (n: Z) (PreH1 : ((Znth i (c_string (input)) 0) > 90)) (PreH2 : ((Znth i (c_string (input)) 0) >= 65)) (PreH3 : (i < n)) (PreH4 : (n = (string_length (input)))) (PreH5 : (out <> 0)) (PreH6 : (0 <= i)) (PreH7 : (i <= n)) (PreH8 : (0 <= nletter)) (PreH9 : (nletter <= i)) (PreH10 : (0 <= w)) (PreH11 : (w <= 127)) (PreH12 : (flip_scan_state_z_161 input output i nletter )) (PreH13 : (valid_string input )) (PreH14 : (problem_161_pre_z input )) (PreH15 : (ascii_range_z input )) (PreH16 : ((string_length (input)) < INT_MAX)) ,
+  ((( &( "s" ) )) # Ptr  |-> s_pre)
+  **  ((( &( "n" ) )) # Int  |-> n)
+  **  ((( &( "out" ) )) # Ptr  |-> out)
+  **  ((( &( "i" ) )) # Int  |-> i)
+  **  ((( &( "nletter" ) )) # Int  |-> nletter)
+  **  ((( &( "w" ) )) # Int  |-> (Znth i (c_string (input)) 0))
+  **  (store_string s_pre input )
+  **  (CharArray.full out i output )
+  **  (CharArray.undef_seg out i (n + 1 ) )
+|--
+  “ (97 <= INT_MAX) ” 
+  &&  “ ((INT_MIN) <= 97) ”
+.
+
+Definition solve_safety_wit_14 := 
+forall (s_pre: Z) (input: (@list Z)) (output: (@list Z)) (w: Z) (nletter: Z) (i: Z) (out: Z) (n: Z) (PreH1 : ((Znth i (c_string (input)) 0) >= 97)) (PreH2 : ((Znth i (c_string (input)) 0) < 65)) (PreH3 : (i < n)) (PreH4 : (n = (string_length (input)))) (PreH5 : (out <> 0)) (PreH6 : (0 <= i)) (PreH7 : (i <= n)) (PreH8 : (0 <= nletter)) (PreH9 : (nletter <= i)) (PreH10 : (0 <= w)) (PreH11 : (w <= 127)) (PreH12 : (flip_scan_state_z_161 input output i nletter )) (PreH13 : (valid_string input )) (PreH14 : (problem_161_pre_z input )) (PreH15 : (ascii_range_z input )) (PreH16 : ((string_length (input)) < INT_MAX)) ,
+  ((( &( "s" ) )) # Ptr  |-> s_pre)
+  **  ((( &( "n" ) )) # Int  |-> n)
+  **  ((( &( "out" ) )) # Ptr  |-> out)
+  **  ((( &( "i" ) )) # Int  |-> i)
+  **  ((( &( "nletter" ) )) # Int  |-> nletter)
+  **  ((( &( "w" ) )) # Int  |-> (Znth i (c_string (input)) 0))
+  **  (store_string s_pre input )
+  **  (CharArray.full out i output )
+  **  (CharArray.undef_seg out i (n + 1 ) )
+|--
+  “ False ”
+.
+
+Definition solve_safety_wit_15 := 
+forall (s_pre: Z) (input: (@list Z)) (output: (@list Z)) (w: Z) (nletter: Z) (i: Z) (out: Z) (n: Z) (PreH1 : ((Znth i (c_string (input)) 0) >= 97)) (PreH2 : ((Znth i (c_string (input)) 0) > 90)) (PreH3 : ((Znth i (c_string (input)) 0) >= 65)) (PreH4 : (i < n)) (PreH5 : (n = (string_length (input)))) (PreH6 : (out <> 0)) (PreH7 : (0 <= i)) (PreH8 : (i <= n)) (PreH9 : (0 <= nletter)) (PreH10 : (nletter <= i)) (PreH11 : (0 <= w)) (PreH12 : (w <= 127)) (PreH13 : (flip_scan_state_z_161 input output i nletter )) (PreH14 : (valid_string input )) (PreH15 : (problem_161_pre_z input )) (PreH16 : (ascii_range_z input )) (PreH17 : ((string_length (input)) < INT_MAX)) ,
+  ((( &( "s" ) )) # Ptr  |-> s_pre)
+  **  ((( &( "n" ) )) # Int  |-> n)
+  **  ((( &( "out" ) )) # Ptr  |-> out)
+  **  ((( &( "i" ) )) # Int  |-> i)
+  **  ((( &( "nletter" ) )) # Int  |-> nletter)
+  **  ((( &( "w" ) )) # Int  |-> (Znth i (c_string (input)) 0))
+  **  (store_string s_pre input )
+  **  (CharArray.full out i output )
+  **  (CharArray.undef_seg out i (n + 1 ) )
+|--
+  “ (122 <= INT_MAX) ” 
+  &&  “ ((INT_MIN) <= 122) ”
+.
+
+Definition solve_safety_wit_16 := 
+forall (s_pre: Z) (input: (@list Z)) (output: (@list Z)) (w: Z) (nletter: Z) (i: Z) (out: Z) (n: Z) (PreH1 : ((Znth i (c_string (input)) 0) <= 122)) (PreH2 : ((Znth i (c_string (input)) 0) >= 97)) (PreH3 : ((Znth i (c_string (input)) 0) > 90)) (PreH4 : ((Znth i (c_string (input)) 0) >= 65)) (PreH5 : (i < n)) (PreH6 : (n = (string_length (input)))) (PreH7 : (out <> 0)) (PreH8 : (0 <= i)) (PreH9 : (i <= n)) (PreH10 : (0 <= nletter)) (PreH11 : (nletter <= i)) (PreH12 : (0 <= w)) (PreH13 : (w <= 127)) (PreH14 : (flip_scan_state_z_161 input output i nletter )) (PreH15 : (valid_string input )) (PreH16 : (problem_161_pre_z input )) (PreH17 : (ascii_range_z input )) (PreH18 : ((string_length (input)) < INT_MAX)) ,
+  ((( &( "s" ) )) # Ptr  |-> s_pre)
+  **  ((( &( "n" ) )) # Int  |-> n)
+  **  ((( &( "out" ) )) # Ptr  |-> out)
+  **  ((( &( "i" ) )) # Int  |-> i)
+  **  ((( &( "nletter" ) )) # Int  |-> nletter)
+  **  ((( &( "w" ) )) # Int  |-> (Znth i (c_string (input)) 0))
+  **  (store_string s_pre input )
+  **  (CharArray.full out i output )
+  **  (CharArray.undef_seg out i (n + 1 ) )
+|--
+  “ (((Znth i (c_string (input)) 0) - 32 ) <= INT_MAX) ” 
+  &&  “ ((INT_MIN) <= ((Znth i (c_string (input)) 0) - 32 )) ”
+.
+
+Definition solve_safety_wit_17 := 
+forall (s_pre: Z) (input: (@list Z)) (output: (@list Z)) (w: Z) (nletter: Z) (i: Z) (out: Z) (n: Z) (PreH1 : ((Znth i (c_string (input)) 0) <= 122)) (PreH2 : ((Znth i (c_string (input)) 0) >= 97)) (PreH3 : ((Znth i (c_string (input)) 0) > 90)) (PreH4 : ((Znth i (c_string (input)) 0) >= 65)) (PreH5 : (i < n)) (PreH6 : (n = (string_length (input)))) (PreH7 : (out <> 0)) (PreH8 : (0 <= i)) (PreH9 : (i <= n)) (PreH10 : (0 <= nletter)) (PreH11 : (nletter <= i)) (PreH12 : (0 <= w)) (PreH13 : (w <= 127)) (PreH14 : (flip_scan_state_z_161 input output i nletter )) (PreH15 : (valid_string input )) (PreH16 : (problem_161_pre_z input )) (PreH17 : (ascii_range_z input )) (PreH18 : ((string_length (input)) < INT_MAX)) ,
+  ((( &( "s" ) )) # Ptr  |-> s_pre)
+  **  ((( &( "n" ) )) # Int  |-> n)
+  **  ((( &( "out" ) )) # Ptr  |-> out)
+  **  ((( &( "i" ) )) # Int  |-> i)
+  **  ((( &( "nletter" ) )) # Int  |-> nletter)
+  **  ((( &( "w" ) )) # Int  |-> (Znth i (c_string (input)) 0))
+  **  (store_string s_pre input )
+  **  (CharArray.full out i output )
+  **  (CharArray.undef_seg out i (n + 1 ) )
+|--
+  “ (32 <= INT_MAX) ” 
+  &&  “ ((INT_MIN) <= 32) ”
+.
+
+Definition solve_safety_wit_18 := 
+forall (s_pre: Z) (input: (@list Z)) (output: (@list Z)) (w: Z) (nletter: Z) (i: Z) (out: Z) (n: Z) (PreH1 : ((Znth i (c_string (input)) 0) < 97)) (PreH2 : ((Znth i (c_string (input)) 0) > 90)) (PreH3 : ((Znth i (c_string (input)) 0) >= 65)) (PreH4 : (i < n)) (PreH5 : (n = (string_length (input)))) (PreH6 : (out <> 0)) (PreH7 : (0 <= i)) (PreH8 : (i <= n)) (PreH9 : (0 <= nletter)) (PreH10 : (nletter <= i)) (PreH11 : (0 <= w)) (PreH12 : (w <= 127)) (PreH13 : (flip_scan_state_z_161 input output i nletter )) (PreH14 : (valid_string input )) (PreH15 : (problem_161_pre_z input )) (PreH16 : (ascii_range_z input )) (PreH17 : ((string_length (input)) < INT_MAX)) ,
+  ((( &( "s" ) )) # Ptr  |-> s_pre)
+  **  ((( &( "n" ) )) # Int  |-> n)
+  **  ((( &( "out" ) )) # Ptr  |-> out)
+  **  ((( &( "i" ) )) # Int  |-> i)
+  **  ((( &( "nletter" ) )) # Int  |-> nletter)
+  **  ((( &( "w" ) )) # Int  |-> (Znth i (c_string (input)) 0))
+  **  (store_string s_pre input )
+  **  (CharArray.full out i output )
+  **  (CharArray.undef_seg out i (n + 1 ) )
+|--
+  “ ((nletter + 1 ) <= INT_MAX) ” 
+  &&  “ ((INT_MIN) <= (nletter + 1 )) ”
+.
+
+Definition solve_safety_wit_19 := 
+forall (s_pre: Z) (input: (@list Z)) (output: (@list Z)) (w: Z) (nletter: Z) (i: Z) (out: Z) (n: Z) (PreH1 : ((Znth i (c_string (input)) 0) < 97)) (PreH2 : ((Znth i (c_string (input)) 0) > 90)) (PreH3 : ((Znth i (c_string (input)) 0) >= 65)) (PreH4 : (i < n)) (PreH5 : (n = (string_length (input)))) (PreH6 : (out <> 0)) (PreH7 : (0 <= i)) (PreH8 : (i <= n)) (PreH9 : (0 <= nletter)) (PreH10 : (nletter <= i)) (PreH11 : (0 <= w)) (PreH12 : (w <= 127)) (PreH13 : (flip_scan_state_z_161 input output i nletter )) (PreH14 : (valid_string input )) (PreH15 : (problem_161_pre_z input )) (PreH16 : (ascii_range_z input )) (PreH17 : ((string_length (input)) < INT_MAX)) ,
+  ((( &( "s" ) )) # Ptr  |-> s_pre)
+  **  ((( &( "n" ) )) # Int  |-> n)
+  **  ((( &( "out" ) )) # Ptr  |-> out)
+  **  ((( &( "i" ) )) # Int  |-> i)
+  **  ((( &( "nletter" ) )) # Int  |-> nletter)
+  **  ((( &( "w" ) )) # Int  |-> (Znth i (c_string (input)) 0))
+  **  (store_string s_pre input )
+  **  (CharArray.full out i output )
+  **  (CharArray.undef_seg out i (n + 1 ) )
+|--
+  “ (1 <= INT_MAX) ” 
+  &&  “ ((INT_MIN) <= 1) ”
+.
+
+Definition solve_safety_wit_20 := 
+forall (s_pre: Z) (input: (@list Z)) (output: (@list Z)) (w: Z) (nletter: Z) (i: Z) (out: Z) (n: Z) (PreH1 : ((Znth i (c_string (input)) 0) < 97)) (PreH2 : ((Znth i (c_string (input)) 0) < 65)) (PreH3 : (i < n)) (PreH4 : (n = (string_length (input)))) (PreH5 : (out <> 0)) (PreH6 : (0 <= i)) (PreH7 : (i <= n)) (PreH8 : (0 <= nletter)) (PreH9 : (nletter <= i)) (PreH10 : (0 <= w)) (PreH11 : (w <= 127)) (PreH12 : (flip_scan_state_z_161 input output i nletter )) (PreH13 : (valid_string input )) (PreH14 : (problem_161_pre_z input )) (PreH15 : (ascii_range_z input )) (PreH16 : ((string_length (input)) < INT_MAX)) ,
+  ((( &( "s" ) )) # Ptr  |-> s_pre)
+  **  ((( &( "n" ) )) # Int  |-> n)
+  **  ((( &( "out" ) )) # Ptr  |-> out)
+  **  ((( &( "i" ) )) # Int  |-> i)
+  **  ((( &( "nletter" ) )) # Int  |-> nletter)
+  **  ((( &( "w" ) )) # Int  |-> (Znth i (c_string (input)) 0))
+  **  (store_string s_pre input )
+  **  (CharArray.full out i output )
+  **  (CharArray.undef_seg out i (n + 1 ) )
+|--
+  “ ((nletter + 1 ) <= INT_MAX) ” 
+  &&  “ ((INT_MIN) <= (nletter + 1 )) ”
+.
+
+Definition solve_safety_wit_21 := 
+forall (s_pre: Z) (input: (@list Z)) (output: (@list Z)) (w: Z) (nletter: Z) (i: Z) (out: Z) (n: Z) (PreH1 : ((Znth i (c_string (input)) 0) < 97)) (PreH2 : ((Znth i (c_string (input)) 0) < 65)) (PreH3 : (i < n)) (PreH4 : (n = (string_length (input)))) (PreH5 : (out <> 0)) (PreH6 : (0 <= i)) (PreH7 : (i <= n)) (PreH8 : (0 <= nletter)) (PreH9 : (nletter <= i)) (PreH10 : (0 <= w)) (PreH11 : (w <= 127)) (PreH12 : (flip_scan_state_z_161 input output i nletter )) (PreH13 : (valid_string input )) (PreH14 : (problem_161_pre_z input )) (PreH15 : (ascii_range_z input )) (PreH16 : ((string_length (input)) < INT_MAX)) ,
+  ((( &( "s" ) )) # Ptr  |-> s_pre)
+  **  ((( &( "n" ) )) # Int  |-> n)
+  **  ((( &( "out" ) )) # Ptr  |-> out)
+  **  ((( &( "i" ) )) # Int  |-> i)
+  **  ((( &( "nletter" ) )) # Int  |-> nletter)
+  **  ((( &( "w" ) )) # Int  |-> (Znth i (c_string (input)) 0))
+  **  (store_string s_pre input )
+  **  (CharArray.full out i output )
+  **  (CharArray.undef_seg out i (n + 1 ) )
+|--
+  “ (1 <= INT_MAX) ” 
+  &&  “ ((INT_MIN) <= 1) ”
+.
+
+Definition solve_safety_wit_22 := 
+forall (s_pre: Z) (input: (@list Z)) (output: (@list Z)) (w: Z) (nletter: Z) (i: Z) (out: Z) (n: Z) (PreH1 : ((Znth i (c_string (input)) 0) > 122)) (PreH2 : ((Znth i (c_string (input)) 0) >= 97)) (PreH3 : ((Znth i (c_string (input)) 0) > 90)) (PreH4 : ((Znth i (c_string (input)) 0) >= 65)) (PreH5 : (i < n)) (PreH6 : (n = (string_length (input)))) (PreH7 : (out <> 0)) (PreH8 : (0 <= i)) (PreH9 : (i <= n)) (PreH10 : (0 <= nletter)) (PreH11 : (nletter <= i)) (PreH12 : (0 <= w)) (PreH13 : (w <= 127)) (PreH14 : (flip_scan_state_z_161 input output i nletter )) (PreH15 : (valid_string input )) (PreH16 : (problem_161_pre_z input )) (PreH17 : (ascii_range_z input )) (PreH18 : ((string_length (input)) < INT_MAX)) ,
+  ((( &( "s" ) )) # Ptr  |-> s_pre)
+  **  ((( &( "n" ) )) # Int  |-> n)
+  **  ((( &( "out" ) )) # Ptr  |-> out)
+  **  ((( &( "i" ) )) # Int  |-> i)
+  **  ((( &( "nletter" ) )) # Int  |-> nletter)
+  **  ((( &( "w" ) )) # Int  |-> (Znth i (c_string (input)) 0))
+  **  (store_string s_pre input )
+  **  (CharArray.full out i output )
+  **  (CharArray.undef_seg out i (n + 1 ) )
+|--
+  “ ((nletter + 1 ) <= INT_MAX) ” 
+  &&  “ ((INT_MIN) <= (nletter + 1 )) ”
+.
+
+Definition solve_safety_wit_23 := 
+forall (s_pre: Z) (input: (@list Z)) (output: (@list Z)) (w: Z) (nletter: Z) (i: Z) (out: Z) (n: Z) (PreH1 : ((Znth i (c_string (input)) 0) > 122)) (PreH2 : ((Znth i (c_string (input)) 0) >= 97)) (PreH3 : ((Znth i (c_string (input)) 0) > 90)) (PreH4 : ((Znth i (c_string (input)) 0) >= 65)) (PreH5 : (i < n)) (PreH6 : (n = (string_length (input)))) (PreH7 : (out <> 0)) (PreH8 : (0 <= i)) (PreH9 : (i <= n)) (PreH10 : (0 <= nletter)) (PreH11 : (nletter <= i)) (PreH12 : (0 <= w)) (PreH13 : (w <= 127)) (PreH14 : (flip_scan_state_z_161 input output i nletter )) (PreH15 : (valid_string input )) (PreH16 : (problem_161_pre_z input )) (PreH17 : (ascii_range_z input )) (PreH18 : ((string_length (input)) < INT_MAX)) ,
+  ((( &( "s" ) )) # Ptr  |-> s_pre)
+  **  ((( &( "n" ) )) # Int  |-> n)
+  **  ((( &( "out" ) )) # Ptr  |-> out)
+  **  ((( &( "i" ) )) # Int  |-> i)
+  **  ((( &( "nletter" ) )) # Int  |-> nletter)
+  **  ((( &( "w" ) )) # Int  |-> (Znth i (c_string (input)) 0))
+  **  (store_string s_pre input )
+  **  (CharArray.full out i output )
+  **  (CharArray.undef_seg out i (n + 1 ) )
+|--
+  “ (1 <= INT_MAX) ” 
+  &&  “ ((INT_MIN) <= 1) ”
+.
+
+Definition solve_safety_wit_24 := 
+forall (s_pre: Z) (input: (@list Z)) (output: (@list Z)) (n: Z) (out: Z) (i: Z) (nletter: Z) (w: Z) (PreH1 : (n = (string_length (input)))) (PreH2 : (out <> 0)) (PreH3 : (0 <= i)) (PreH4 : (i < n)) (PreH5 : (0 <= nletter)) (PreH6 : (nletter <= (i + 1 ))) (PreH7 : (0 <= w)) (PreH8 : (w <= 127)) (PreH9 : (flip_scan_state_z_161 input output (i + 1 ) nletter )) (PreH10 : (valid_string input )) (PreH11 : (problem_161_pre_z input )) (PreH12 : (ascii_range_z input )) (PreH13 : ((string_length (input)) < INT_MAX)) ,
+  ((( &( "s" ) )) # Ptr  |-> s_pre)
+  **  ((( &( "n" ) )) # Int  |-> n)
+  **  ((( &( "out" ) )) # Ptr  |-> out)
+  **  ((( &( "i" ) )) # Int  |-> i)
+  **  ((( &( "nletter" ) )) # Int  |-> nletter)
+  **  ((( &( "w" ) )) # Int  |-> w)
+  **  (store_string s_pre input )
+  **  (CharArray.full out (i + 1 ) output )
+  **  (CharArray.undef_seg out (i + 1 ) (n + 1 ) )
+|--
+  “ ((i + 1 ) <= INT_MAX) ” 
+  &&  “ ((INT_MIN) <= (i + 1 )) ”
+.
+
+Definition solve_safety_wit_25 := 
+forall (s_pre: Z) (input: (@list Z)) (output: (@list Z)) (n: Z) (i: Z) (out: Z) (nletter: Z) (w: Z) (PreH1 : (n = (string_length (input)))) (PreH2 : (i = n)) (PreH3 : (out <> 0)) (PreH4 : (0 <= nletter)) (PreH5 : (nletter <= n)) (PreH6 : (flip_scan_state_z_161 input output n nletter )) (PreH7 : (valid_string input )) (PreH8 : (problem_161_pre_z input )) (PreH9 : (ascii_range_z input )) (PreH10 : ((string_length (input)) < INT_MAX)) ,
+  ((( &( "s" ) )) # Ptr  |-> s_pre)
+  **  ((( &( "n" ) )) # Int  |-> n)
+  **  ((( &( "i" ) )) # Int  |-> i)
+  **  ((( &( "out" ) )) # Ptr  |-> out)
+  **  ((( &( "nletter" ) )) # Int  |-> nletter)
+  **  ((( &( "w" ) )) # Int  |-> w)
+  **  (store_string s_pre input )
+  **  (CharArray.full out n output )
+  **  (CharArray.undef_seg out n (n + 1 ) )
+|--
+  “ (0 <= INT_MAX) ” 
+  &&  “ ((INT_MIN) <= 0) ”
+.
+
+Definition solve_safety_wit_26 := 
+forall (s_pre: Z) (input: (@list Z)) (output: (@list Z)) (n: Z) (i: Z) (out: Z) (nletter: Z) (w: Z) (PreH1 : (n = (string_length (input)))) (PreH2 : (i = n)) (PreH3 : (out <> 0)) (PreH4 : (nletter = n)) (PreH5 : (no_letter_z_161 input )) (PreH6 : (flip_output_z_161 input output )) (PreH7 : (valid_string input )) (PreH8 : (valid_string output )) (PreH9 : (problem_161_pre_z input )) (PreH10 : (ascii_range_z input )) (PreH11 : ((string_length (input)) < INT_MAX)) ,
+  ((( &( "p" ) )) # Ptr  |->_)
+  **  ((( &( "s" ) )) # Ptr  |-> s_pre)
+  **  ((( &( "n" ) )) # Int  |-> n)
+  **  ((( &( "i" ) )) # Int  |-> i)
+  **  ((( &( "out" ) )) # Ptr  |-> out)
+  **  ((( &( "nletter" ) )) # Int  |-> nletter)
+  **  ((( &( "w" ) )) # Int  |-> w)
+  **  (store_string s_pre input )
+  **  (CharArray.full out (n + 1 ) (c_string (output)) )
+|--
+  “ ((n + 1 ) <= INT_MAX) ” 
+  &&  “ ((INT_MIN) <= (n + 1 )) ”
+.
+
+Definition solve_safety_wit_27 := 
+forall (s_pre: Z) (input: (@list Z)) (output: (@list Z)) (n: Z) (i: Z) (out: Z) (nletter: Z) (w: Z) (PreH1 : (n = (string_length (input)))) (PreH2 : (i = n)) (PreH3 : (out <> 0)) (PreH4 : (nletter = n)) (PreH5 : (no_letter_z_161 input )) (PreH6 : (flip_output_z_161 input output )) (PreH7 : (valid_string input )) (PreH8 : (valid_string output )) (PreH9 : (problem_161_pre_z input )) (PreH10 : (ascii_range_z input )) (PreH11 : ((string_length (input)) < INT_MAX)) ,
+  ((( &( "p" ) )) # Ptr  |->_)
+  **  ((( &( "s" ) )) # Ptr  |-> s_pre)
+  **  ((( &( "n" ) )) # Int  |-> n)
+  **  ((( &( "i" ) )) # Int  |-> i)
+  **  ((( &( "out" ) )) # Ptr  |-> out)
+  **  ((( &( "nletter" ) )) # Int  |-> nletter)
+  **  ((( &( "w" ) )) # Int  |-> w)
+  **  (store_string s_pre input )
+  **  (CharArray.full out (n + 1 ) (c_string (output)) )
+|--
+  “ (1 <= INT_MAX) ” 
+  &&  “ ((INT_MIN) <= 1) ”
+.
+
+Definition solve_safety_wit_28 := 
+forall (s_pre: Z) (input: (@list Z)) (output: (@list Z)) (n: Z) (i: Z) (out: Z) (nletter: Z) (w: Z) (retval: Z) (PreH1 : (retval <> 0)) (PreH2 : (0 <= ((string_length (input)) + 1 ))) (PreH3 : (0 <= (n + 1 ))) (PreH4 : (n = (string_length (input)))) (PreH5 : (i = n)) (PreH6 : (out <> 0)) (PreH7 : (nletter = n)) (PreH8 : (no_letter_z_161 input )) (PreH9 : (flip_output_z_161 input output )) (PreH10 : (valid_string input )) (PreH11 : (valid_string output )) (PreH12 : (problem_161_pre_z input )) (PreH13 : (ascii_range_z input )) (PreH14 : ((string_length (input)) < INT_MAX)) ,
+  (CharArray.undef_full retval (n + 1 ) )
+  **  (CharArray.full s_pre ((string_length (input)) + 1 ) (c_string (input)) )
+  **  ((( &( "p" ) )) # Ptr  |-> retval)
+  **  ((( &( "s" ) )) # Ptr  |-> s_pre)
+  **  ((( &( "n" ) )) # Int  |-> n)
+  **  ((( &( "i" ) )) # Int  |-> i)
+  **  ((( &( "out" ) )) # Ptr  |-> out)
+  **  ((( &( "nletter" ) )) # Int  |-> nletter)
+  **  ((( &( "w" ) )) # Int  |-> w)
+  **  (CharArray.full out (n + 1 ) (c_string (output)) )
+|--
+  “ (0 <= INT_MAX) ” 
+  &&  “ ((INT_MIN) <= 0) ”
+.
+
+Definition solve_safety_wit_29 := 
+forall (s_pre: Z) (input: (@list Z)) (output: (@list Z)) (n: Z) (i: Z) (out: Z) (nletter: Z) (w: Z) (retval: Z) (PreH1 : (retval = 0)) (PreH2 : (retval <> 0)) (PreH3 : (0 <= ((string_length (input)) + 1 ))) (PreH4 : (0 <= (n + 1 ))) (PreH5 : (n = (string_length (input)))) (PreH6 : (i = n)) (PreH7 : (out <> 0)) (PreH8 : (nletter = n)) (PreH9 : (no_letter_z_161 input )) (PreH10 : (flip_output_z_161 input output )) (PreH11 : (valid_string input )) (PreH12 : (valid_string output )) (PreH13 : (problem_161_pre_z input )) (PreH14 : (ascii_range_z input )) (PreH15 : ((string_length (input)) < INT_MAX)) ,
+  (CharArray.undef_full retval (n + 1 ) )
+  **  (CharArray.full s_pre ((string_length (input)) + 1 ) (c_string (input)) )
+  **  ((( &( "p" ) )) # Ptr  |-> retval)
+  **  ((( &( "s" ) )) # Ptr  |-> s_pre)
+  **  ((( &( "n" ) )) # Int  |-> n)
+  **  ((( &( "i" ) )) # Int  |-> i)
+  **  ((( &( "out" ) )) # Ptr  |-> out)
+  **  ((( &( "nletter" ) )) # Int  |-> nletter)
+  **  ((( &( "w" ) )) # Int  |-> w)
+  **  (CharArray.full out (n + 1 ) (c_string (output)) )
+|--
+  “ False ”
+.
+
+Definition solve_safety_wit_30 := 
+forall (s_pre: Z) (input: (@list Z)) (output: (@list Z)) (n: Z) (i: Z) (out: Z) (nletter: Z) (w: Z) (retval: Z) (PreH1 : (retval <> 0)) (PreH2 : (retval <> 0)) (PreH3 : (0 <= ((string_length (input)) + 1 ))) (PreH4 : (0 <= (n + 1 ))) (PreH5 : (n = (string_length (input)))) (PreH6 : (i = n)) (PreH7 : (out <> 0)) (PreH8 : (nletter = n)) (PreH9 : (no_letter_z_161 input )) (PreH10 : (flip_output_z_161 input output )) (PreH11 : (valid_string input )) (PreH12 : (valid_string output )) (PreH13 : (problem_161_pre_z input )) (PreH14 : (ascii_range_z input )) (PreH15 : ((string_length (input)) < INT_MAX)) ,
+  ((( &( "j" ) )) # Int  |->_)
+  **  (CharArray.undef_full retval (n + 1 ) )
+  **  (CharArray.full s_pre ((string_length (input)) + 1 ) (c_string (input)) )
+  **  ((( &( "p" ) )) # Ptr  |-> retval)
+  **  ((( &( "s" ) )) # Ptr  |-> s_pre)
+  **  ((( &( "n" ) )) # Int  |-> n)
+  **  ((( &( "i" ) )) # Int  |-> i)
+  **  ((( &( "out" ) )) # Ptr  |-> out)
+  **  ((( &( "nletter" ) )) # Int  |-> nletter)
+  **  ((( &( "w" ) )) # Int  |-> w)
+  **  (CharArray.full out (n + 1 ) (c_string (output)) )
+|--
+  “ (0 <= INT_MAX) ” 
+  &&  “ ((INT_MIN) <= 0) ”
+.
+
+Definition solve_safety_wit_31 := 
+forall (s_pre: Z) (input: (@list Z)) (rev_output: (@list Z)) (output: (@list Z)) (j: Z) (w: Z) (nletter: Z) (p: Z) (out: Z) (i: Z) (n: Z) (PreH1 : (j < n)) (PreH2 : (n = (string_length (input)))) (PreH3 : (i = n)) (PreH4 : (out <> 0)) (PreH5 : (p <> 0)) (PreH6 : (nletter = n)) (PreH7 : (0 <= j)) (PreH8 : (j <= n)) (PreH9 : (no_letter_z_161 input )) (PreH10 : (flip_output_z_161 input output )) (PreH11 : (reverse_scan_state_z_161 input rev_output j )) (PreH12 : (valid_string input )) (PreH13 : (valid_string output )) (PreH14 : (problem_161_pre_z input )) (PreH15 : (ascii_range_z input )) (PreH16 : ((string_length (input)) < INT_MAX)) ,
+  ((( &( "s" ) )) # Ptr  |-> s_pre)
+  **  ((( &( "n" ) )) # Int  |-> n)
+  **  ((( &( "i" ) )) # Int  |-> i)
+  **  ((( &( "out" ) )) # Ptr  |-> out)
+  **  ((( &( "p" ) )) # Ptr  |-> p)
+  **  ((( &( "nletter" ) )) # Int  |-> nletter)
+  **  ((( &( "w" ) )) # Int  |-> w)
+  **  ((( &( "j" ) )) # Int  |-> j)
+  **  (store_string s_pre input )
+  **  (CharArray.full out (n + 1 ) (c_string (output)) )
+  **  (CharArray.full p j rev_output )
+  **  (CharArray.undef_seg p j (n + 1 ) )
+|--
+  “ (((n - 1 ) - j ) <= INT_MAX) ” 
+  &&  “ ((INT_MIN) <= ((n - 1 ) - j )) ”
+.
+
+Definition solve_safety_wit_32 := 
+forall (s_pre: Z) (input: (@list Z)) (rev_output: (@list Z)) (output: (@list Z)) (j: Z) (w: Z) (nletter: Z) (p: Z) (out: Z) (i: Z) (n: Z) (PreH1 : (j < n)) (PreH2 : (n = (string_length (input)))) (PreH3 : (i = n)) (PreH4 : (out <> 0)) (PreH5 : (p <> 0)) (PreH6 : (nletter = n)) (PreH7 : (0 <= j)) (PreH8 : (j <= n)) (PreH9 : (no_letter_z_161 input )) (PreH10 : (flip_output_z_161 input output )) (PreH11 : (reverse_scan_state_z_161 input rev_output j )) (PreH12 : (valid_string input )) (PreH13 : (valid_string output )) (PreH14 : (problem_161_pre_z input )) (PreH15 : (ascii_range_z input )) (PreH16 : ((string_length (input)) < INT_MAX)) ,
+  ((( &( "s" ) )) # Ptr  |-> s_pre)
+  **  ((( &( "n" ) )) # Int  |-> n)
+  **  ((( &( "i" ) )) # Int  |-> i)
+  **  ((( &( "out" ) )) # Ptr  |-> out)
+  **  ((( &( "p" ) )) # Ptr  |-> p)
+  **  ((( &( "nletter" ) )) # Int  |-> nletter)
+  **  ((( &( "w" ) )) # Int  |-> w)
+  **  ((( &( "j" ) )) # Int  |-> j)
+  **  (store_string s_pre input )
+  **  (CharArray.full out (n + 1 ) (c_string (output)) )
+  **  (CharArray.full p j rev_output )
+  **  (CharArray.undef_seg p j (n + 1 ) )
+|--
+  “ ((n - 1 ) <= INT_MAX) ” 
+  &&  “ ((INT_MIN) <= (n - 1 )) ”
+.
+
+Definition solve_safety_wit_33 := 
+forall (s_pre: Z) (input: (@list Z)) (rev_output: (@list Z)) (output: (@list Z)) (j: Z) (w: Z) (nletter: Z) (p: Z) (out: Z) (i: Z) (n: Z) (PreH1 : (j < n)) (PreH2 : (n = (string_length (input)))) (PreH3 : (i = n)) (PreH4 : (out <> 0)) (PreH5 : (p <> 0)) (PreH6 : (nletter = n)) (PreH7 : (0 <= j)) (PreH8 : (j <= n)) (PreH9 : (no_letter_z_161 input )) (PreH10 : (flip_output_z_161 input output )) (PreH11 : (reverse_scan_state_z_161 input rev_output j )) (PreH12 : (valid_string input )) (PreH13 : (valid_string output )) (PreH14 : (problem_161_pre_z input )) (PreH15 : (ascii_range_z input )) (PreH16 : ((string_length (input)) < INT_MAX)) ,
+  ((( &( "s" ) )) # Ptr  |-> s_pre)
+  **  ((( &( "n" ) )) # Int  |-> n)
+  **  ((( &( "i" ) )) # Int  |-> i)
+  **  ((( &( "out" ) )) # Ptr  |-> out)
+  **  ((( &( "p" ) )) # Ptr  |-> p)
+  **  ((( &( "nletter" ) )) # Int  |-> nletter)
+  **  ((( &( "w" ) )) # Int  |-> w)
+  **  ((( &( "j" ) )) # Int  |-> j)
+  **  (store_string s_pre input )
+  **  (CharArray.full out (n + 1 ) (c_string (output)) )
+  **  (CharArray.full p j rev_output )
+  **  (CharArray.undef_seg p j (n + 1 ) )
+|--
+  “ (1 <= INT_MAX) ” 
+  &&  “ ((INT_MIN) <= 1) ”
+.
+
+Definition solve_safety_wit_34 := 
+forall (s_pre: Z) (input: (@list Z)) (output: (@list Z)) (rev_output: (@list Z)) (n: Z) (i: Z) (out: Z) (p: Z) (nletter: Z) (w: Z) (j: Z) (PreH1 : (n = (string_length (input)))) (PreH2 : (i = n)) (PreH3 : (out <> 0)) (PreH4 : (p <> 0)) (PreH5 : (nletter = n)) (PreH6 : (0 <= j)) (PreH7 : (j < n)) (PreH8 : (no_letter_z_161 input )) (PreH9 : (flip_output_z_161 input output )) (PreH10 : (reverse_scan_state_z_161 input rev_output (j + 1 ) )) (PreH11 : (valid_string input )) (PreH12 : (valid_string output )) (PreH13 : (problem_161_pre_z input )) (PreH14 : (ascii_range_z input )) (PreH15 : ((string_length (input)) < INT_MAX)) ,
+  ((( &( "s" ) )) # Ptr  |-> s_pre)
+  **  ((( &( "n" ) )) # Int  |-> n)
+  **  ((( &( "i" ) )) # Int  |-> i)
+  **  ((( &( "out" ) )) # Ptr  |-> out)
+  **  ((( &( "p" ) )) # Ptr  |-> p)
+  **  ((( &( "nletter" ) )) # Int  |-> nletter)
+  **  ((( &( "w" ) )) # Int  |-> w)
+  **  ((( &( "j" ) )) # Int  |-> j)
+  **  (store_string s_pre input )
+  **  (CharArray.full out (n + 1 ) (c_string (output)) )
+  **  (CharArray.full p (j + 1 ) rev_output )
+  **  (CharArray.undef_seg p (j + 1 ) (n + 1 ) )
+|--
+  “ ((j + 1 ) <= INT_MAX) ” 
+  &&  “ ((INT_MIN) <= (j + 1 )) ”
+.
+
+Definition solve_safety_wit_35 := 
+forall (s_pre: Z) (input: (@list Z)) (output: (@list Z)) (rev_output: (@list Z)) (n: Z) (i: Z) (j: Z) (out: Z) (p: Z) (nletter: Z) (w: Z) (PreH1 : (n = (string_length (input)))) (PreH2 : (i = n)) (PreH3 : (j = n)) (PreH4 : (out <> 0)) (PreH5 : (p <> 0)) (PreH6 : (nletter = n)) (PreH7 : (no_letter_z_161 input )) (PreH8 : (flip_output_z_161 input output )) (PreH9 : (reverse_output_z_161 input rev_output )) (PreH10 : (valid_string input )) (PreH11 : (valid_string output )) (PreH12 : (valid_string rev_output )) (PreH13 : (problem_161_pre_z input )) (PreH14 : (problem_161_spec_z input rev_output )) (PreH15 : (ascii_range_z input )) (PreH16 : ((string_length (input)) < INT_MAX)) ,
+  ((( &( "s" ) )) # Ptr  |-> s_pre)
+  **  ((( &( "n" ) )) # Int  |-> n)
+  **  ((( &( "i" ) )) # Int  |-> i)
+  **  ((( &( "j" ) )) # Int  |-> j)
+  **  ((( &( "out" ) )) # Ptr  |-> out)
+  **  ((( &( "p" ) )) # Ptr  |-> p)
+  **  ((( &( "nletter" ) )) # Int  |-> nletter)
+  **  ((( &( "w" ) )) # Int  |-> w)
+  **  (store_string s_pre input )
+  **  (CharArray.full out (n + 1 ) (c_string (output)) )
+  **  (CharArray.full p n rev_output )
+  **  (CharArray.undef_seg p n (n + 1 ) )
+|--
+  “ (0 <= INT_MAX) ” 
+  &&  “ ((INT_MIN) <= 0) ”
+.
+
+Definition solve_safety_wit_36 := 
+forall (s_pre: Z) (input: (@list Z)) (output: (@list Z)) (rev_output: (@list Z)) (n: Z) (i: Z) (j: Z) (out: Z) (p: Z) (nletter: Z) (w: Z) (PreH1 : (0 <= ((string_length (input)) + 1 ))) (PreH2 : (0 <= n)) (PreH3 : (0 <= (n + 1 ))) (PreH4 : (n = (string_length (input)))) (PreH5 : (i = n)) (PreH6 : (j = n)) (PreH7 : (out <> 0)) (PreH8 : (p <> 0)) (PreH9 : (nletter = n)) (PreH10 : (no_letter_z_161 input )) (PreH11 : (flip_output_z_161 input output )) (PreH12 : (reverse_output_z_161 input rev_output )) (PreH13 : (valid_string input )) (PreH14 : (valid_string output )) (PreH15 : (valid_string rev_output )) (PreH16 : (problem_161_pre_z input )) (PreH17 : (problem_161_spec_z input rev_output )) (PreH18 : (ascii_range_z input )) (PreH19 : ((string_length (input)) < INT_MAX)) ,
+  (CharArray.full p (n + 1 ) (app (rev_output) ((cons (0) ((@nil Z))))) )
+  **  (CharArray.undef_seg p (n + 1 ) (n + 1 ) )
+  **  (CharArray.full s_pre ((string_length (input)) + 1 ) (c_string (input)) )
+  **  ((( &( "s" ) )) # Ptr  |-> s_pre)
+  **  ((( &( "n" ) )) # Int  |-> n)
+  **  ((( &( "i" ) )) # Int  |-> i)
+  **  ((( &( "j" ) )) # Int  |-> j)
+  **  ((( &( "out" ) )) # Ptr  |-> out)
+  **  ((( &( "p" ) )) # Ptr  |-> p)
+  **  ((( &( "nletter" ) )) # Int  |-> nletter)
+  **  ((( &( "w" ) )) # Int  |-> w)
+  **  (CharArray.full out (n + 1 ) (c_string (output)) )
+|--
+  “ ((n + 1 ) <= INT_MAX) ” 
+  &&  “ ((INT_MIN) <= (n + 1 )) ”
+.
+
+Definition solve_safety_wit_37 := 
+forall (s_pre: Z) (input: (@list Z)) (output: (@list Z)) (rev_output: (@list Z)) (n: Z) (i: Z) (j: Z) (out: Z) (p: Z) (nletter: Z) (w: Z) (PreH1 : (0 <= ((string_length (input)) + 1 ))) (PreH2 : (0 <= n)) (PreH3 : (0 <= (n + 1 ))) (PreH4 : (n = (string_length (input)))) (PreH5 : (i = n)) (PreH6 : (j = n)) (PreH7 : (out <> 0)) (PreH8 : (p <> 0)) (PreH9 : (nletter = n)) (PreH10 : (no_letter_z_161 input )) (PreH11 : (flip_output_z_161 input output )) (PreH12 : (reverse_output_z_161 input rev_output )) (PreH13 : (valid_string input )) (PreH14 : (valid_string output )) (PreH15 : (valid_string rev_output )) (PreH16 : (problem_161_pre_z input )) (PreH17 : (problem_161_spec_z input rev_output )) (PreH18 : (ascii_range_z input )) (PreH19 : ((string_length (input)) < INT_MAX)) ,
+  (CharArray.full p (n + 1 ) (app (rev_output) ((cons (0) ((@nil Z))))) )
+  **  (CharArray.undef_seg p (n + 1 ) (n + 1 ) )
+  **  (CharArray.full s_pre ((string_length (input)) + 1 ) (c_string (input)) )
+  **  ((( &( "s" ) )) # Ptr  |-> s_pre)
+  **  ((( &( "n" ) )) # Int  |-> n)
+  **  ((( &( "i" ) )) # Int  |-> i)
+  **  ((( &( "j" ) )) # Int  |-> j)
+  **  ((( &( "out" ) )) # Ptr  |-> out)
+  **  ((( &( "p" ) )) # Ptr  |-> p)
+  **  ((( &( "nletter" ) )) # Int  |-> nletter)
+  **  ((( &( "w" ) )) # Int  |-> w)
+  **  (CharArray.full out (n + 1 ) (c_string (output)) )
+|--
+  “ (1 <= INT_MAX) ” 
+  &&  “ ((INT_MIN) <= 1) ”
+.
+
+Definition solve_entail_wit_1 := 
+(
+forall (s_pre: Z) (input: (@list Z)) (retval: Z) (retval_2: Z) (PreH1 : (retval_2 <> 0)) (PreH2 : (retval_2 <> 0)) (PreH3 : (retval = (string_length (input)))) (PreH4 : (0 <= ((string_length (input)) + 1 ))) (PreH5 : (valid_string input )) (PreH6 : (problem_161_pre_z input )) (PreH7 : (ascii_range_z input )) (PreH8 : ((string_length (input)) < INT_MAX)) ,
+  (CharArray.undef_full retval_2 (retval + 1 ) )
+  **  (CharArray.full s_pre ((string_length (input)) + 1 ) (c_string (input)) )
+|--
+  EX (output: (@list Z)) ,
+  “ (retval = (string_length (input))) ” 
+  &&  “ (retval_2 <> 0) ” 
+  &&  “ (0 <= 0) ” 
+  &&  “ (0 <= retval) ” 
+  &&  “ (0 <= 0) ” 
+  &&  “ (0 <= 0) ” 
+  &&  “ (0 <= 0) ” 
+  &&  “ (0 <= 127) ” 
+  &&  “ (flip_scan_state_z_161 input output 0 0 ) ” 
+  &&  “ (valid_string input ) ” 
+  &&  “ (problem_161_pre_z input ) ” 
+  &&  “ (ascii_range_z input ) ” 
+  &&  “ ((string_length (input)) < INT_MAX) ”
+  &&  (store_string s_pre input )
+  **  (CharArray.full retval_2 0 output )
+  **  (CharArray.undef_seg retval_2 0 (retval + 1 ) )
+) \/
+(
+forall (input: (@list Z)) (retval: Z) (retval_2: Z) (PreH1 : (retval_2 <> 0)) (PreH2 : (retval_2 <> 0)) (PreH3 : (retval = (string_length (input)))) (PreH4 : (0 <= ((string_length (input)) + 1 ))) (PreH5 : (valid_string input )) (PreH6 : (problem_161_pre_z input )) (PreH7 : (ascii_range_z input )) (PreH8 : ((string_length (input)) < INT_MAX)) ,
+  (CharArray.undef_full retval_2 (retval + 1 ) )
+|--
+  “ (flip_scan_state_z_161 input (@nil Z) 0 0 ) ” 
+  &&  “ (0 <= retval) ”
+  &&  (CharArray.undef_full retval_2 (retval + 1 ) )
+).
+
+Definition solve_entail_wit_1_split_goal_1 := 
+forall (input: (@list Z)) (retval: Z) (retval_2: Z) (PreH1 : (retval_2 <> 0)) (PreH2 : (retval_2 <> 0)) (PreH3 : (retval = (string_length (input)))) (PreH4 : (0 <= ((string_length (input)) + 1 ))) (PreH5 : (valid_string input )) (PreH6 : (problem_161_pre_z input )) (PreH7 : (ascii_range_z input )) (PreH8 : ((string_length (input)) < INT_MAX)) ,
+  (CharArray.undef_full retval_2 (retval + 1 ) )
+|--
+  “ (flip_scan_state_z_161 input (@nil Z) 0 0 ) ”
+.
+
+Definition solve_entail_wit_1_split_goal_2 := 
+forall (input: (@list Z)) (retval: Z) (retval_2: Z) (PreH1 : (retval_2 <> 0)) (PreH2 : (retval_2 <> 0)) (PreH3 : (retval = (string_length (input)))) (PreH4 : (0 <= ((string_length (input)) + 1 ))) (PreH5 : (valid_string input )) (PreH6 : (problem_161_pre_z input )) (PreH7 : (ascii_range_z input )) (PreH8 : ((string_length (input)) < INT_MAX)) ,
+  (CharArray.undef_full retval_2 (retval + 1 ) )
+|--
+  “ (0 <= retval) ”
+.
+
+Definition solve_entail_wit_1_split_goal_spatial := 
+forall (input: (@list Z)) (retval: Z) (retval_2: Z) (PreH1 : (retval_2 <> 0)) (PreH2 : (retval_2 <> 0)) (PreH3 : (retval = (string_length (input)))) (PreH4 : (0 <= ((string_length (input)) + 1 ))) (PreH5 : (valid_string input )) (PreH6 : (problem_161_pre_z input )) (PreH7 : (ascii_range_z input )) (PreH8 : ((string_length (input)) < INT_MAX)) ,
+  (CharArray.undef_full retval_2 (retval + 1 ) )
+|--
+  (CharArray.undef_full retval_2 (retval + 1 ) )
+.
+
+Definition solve_entail_wit_2_1 := 
+(
+forall (s_pre: Z) (input: (@list Z)) (output_2: (@list Z)) (w: Z) (nletter: Z) (i: Z) (out: Z) (n: Z) (PreH1 : (0 <= ((string_length (input)) + 1 ))) (PreH2 : ((Znth i (c_string (input)) 0) > 122)) (PreH3 : ((Znth i (c_string (input)) 0) >= 97)) (PreH4 : ((Znth i (c_string (input)) 0) > 90)) (PreH5 : ((Znth i (c_string (input)) 0) >= 65)) (PreH6 : (i < n)) (PreH7 : (n = (string_length (input)))) (PreH8 : (out <> 0)) (PreH9 : (0 <= i)) (PreH10 : (i <= n)) (PreH11 : (0 <= nletter)) (PreH12 : (nletter <= i)) (PreH13 : (0 <= w)) (PreH14 : (w <= 127)) (PreH15 : (flip_scan_state_z_161 input output_2 i nletter )) (PreH16 : (valid_string input )) (PreH17 : (problem_161_pre_z input )) (PreH18 : (ascii_range_z input )) (PreH19 : ((string_length (input)) < INT_MAX)) ,
+  (CharArray.full out (i + 1 ) (app (output_2) ((cons ((signed_last_nbits ((Znth i (c_string (input)) 0)) (8))) ((@nil Z))))) )
+  **  (CharArray.undef_seg out (i + 1 ) (n + 1 ) )
+  **  (CharArray.full s_pre ((string_length (input)) + 1 ) (c_string (input)) )
+|--
+  EX (output: (@list Z)) ,
+  “ (n = (string_length (input))) ” 
+  &&  “ (out <> 0) ” 
+  &&  “ (0 <= i) ” 
+  &&  “ (i < n) ” 
+  &&  “ (0 <= (nletter + 1 )) ” 
+  &&  “ ((nletter + 1 ) <= (i + 1 )) ” 
+  &&  “ (0 <= (Znth i (c_string (input)) 0)) ” 
+  &&  “ ((Znth i (c_string (input)) 0) <= 127) ” 
+  &&  “ (flip_scan_state_z_161 input output (i + 1 ) (nletter + 1 ) ) ” 
+  &&  “ (valid_string input ) ” 
+  &&  “ (problem_161_pre_z input ) ” 
+  &&  “ (ascii_range_z input ) ” 
+  &&  “ ((string_length (input)) < INT_MAX) ”
+  &&  (store_string s_pre input )
+  **  (CharArray.full out (i + 1 ) output )
+  **  (CharArray.undef_seg out (i + 1 ) (n + 1 ) )
+) \/
+(
+forall (input: (@list Z)) (output_2: (@list Z)) (w: Z) (nletter: Z) (i: Z) (out: Z) (n: Z) (PreH1 : (0 <= ((string_length (input)) + 1 ))) (PreH2 : ((Znth i (c_string (input)) 0) > 122)) (PreH3 : ((Znth i (c_string (input)) 0) >= 97)) (PreH4 : ((Znth i (c_string (input)) 0) > 90)) (PreH5 : ((Znth i (c_string (input)) 0) >= 65)) (PreH6 : (i < n)) (PreH7 : (n = (string_length (input)))) (PreH8 : (out <> 0)) (PreH9 : (0 <= i)) (PreH10 : (i <= n)) (PreH11 : (0 <= nletter)) (PreH12 : (nletter <= i)) (PreH13 : (0 <= w)) (PreH14 : (w <= 127)) (PreH15 : (flip_scan_state_z_161 input output_2 i nletter )) (PreH16 : (valid_string input )) (PreH17 : (problem_161_pre_z input )) (PreH18 : (ascii_range_z input )) (PreH19 : ((string_length (input)) < INT_MAX)) ,
+  TT && emp 
+|--
+  “ (flip_scan_state_z_161 input (app (output_2) ((cons ((signed_last_nbits ((Znth i (c_string (input)) 0)) (8))) ((@nil Z))))) (i + 1 ) (nletter + 1 ) ) ” 
+  &&  “ ((Znth i (c_string (input)) 0) <= 127) ”
+  &&  emp
+).
+
+Definition solve_entail_wit_2_1_split_goal_1 := 
+forall (input: (@list Z)) (output_2: (@list Z)) (w: Z) (nletter: Z) (i: Z) (out: Z) (n: Z) (PreH1 : (0 <= ((string_length (input)) + 1 ))) (PreH2 : ((Znth i (c_string (input)) 0) > 122)) (PreH3 : ((Znth i (c_string (input)) 0) >= 97)) (PreH4 : ((Znth i (c_string (input)) 0) > 90)) (PreH5 : ((Znth i (c_string (input)) 0) >= 65)) (PreH6 : (i < n)) (PreH7 : (n = (string_length (input)))) (PreH8 : (out <> 0)) (PreH9 : (0 <= i)) (PreH10 : (i <= n)) (PreH11 : (0 <= nletter)) (PreH12 : (nletter <= i)) (PreH13 : (0 <= w)) (PreH14 : (w <= 127)) (PreH15 : (flip_scan_state_z_161 input output_2 i nletter )) (PreH16 : (valid_string input )) (PreH17 : (problem_161_pre_z input )) (PreH18 : (ascii_range_z input )) (PreH19 : ((string_length (input)) < INT_MAX)) ,
+  TT && emp 
+|--
+  “ (flip_scan_state_z_161 input (app (output_2) ((cons ((signed_last_nbits ((Znth i (c_string (input)) 0)) (8))) ((@nil Z))))) (i + 1 ) (nletter + 1 ) ) ”
+.
+
+Definition solve_entail_wit_2_1_split_goal_2 := 
+forall (input: (@list Z)) (output_2: (@list Z)) (w: Z) (nletter: Z) (i: Z) (out: Z) (n: Z) (PreH1 : (0 <= ((string_length (input)) + 1 ))) (PreH2 : ((Znth i (c_string (input)) 0) > 122)) (PreH3 : ((Znth i (c_string (input)) 0) >= 97)) (PreH4 : ((Znth i (c_string (input)) 0) > 90)) (PreH5 : ((Znth i (c_string (input)) 0) >= 65)) (PreH6 : (i < n)) (PreH7 : (n = (string_length (input)))) (PreH8 : (out <> 0)) (PreH9 : (0 <= i)) (PreH10 : (i <= n)) (PreH11 : (0 <= nletter)) (PreH12 : (nletter <= i)) (PreH13 : (0 <= w)) (PreH14 : (w <= 127)) (PreH15 : (flip_scan_state_z_161 input output_2 i nletter )) (PreH16 : (valid_string input )) (PreH17 : (problem_161_pre_z input )) (PreH18 : (ascii_range_z input )) (PreH19 : ((string_length (input)) < INT_MAX)) ,
+  TT && emp 
+|--
+  “ ((Znth i (c_string (input)) 0) <= 127) ”
+.
+
+Definition solve_entail_wit_2_2 := 
+(
+forall (s_pre: Z) (input: (@list Z)) (output_2: (@list Z)) (w: Z) (nletter: Z) (i: Z) (out: Z) (n: Z) (PreH1 : (0 <= ((string_length (input)) + 1 ))) (PreH2 : ((Znth i (c_string (input)) 0) < 97)) (PreH3 : ((Znth i (c_string (input)) 0) < 65)) (PreH4 : (i < n)) (PreH5 : (n = (string_length (input)))) (PreH6 : (out <> 0)) (PreH7 : (0 <= i)) (PreH8 : (i <= n)) (PreH9 : (0 <= nletter)) (PreH10 : (nletter <= i)) (PreH11 : (0 <= w)) (PreH12 : (w <= 127)) (PreH13 : (flip_scan_state_z_161 input output_2 i nletter )) (PreH14 : (valid_string input )) (PreH15 : (problem_161_pre_z input )) (PreH16 : (ascii_range_z input )) (PreH17 : ((string_length (input)) < INT_MAX)) ,
+  (CharArray.full out (i + 1 ) (app (output_2) ((cons ((signed_last_nbits ((Znth i (c_string (input)) 0)) (8))) ((@nil Z))))) )
+  **  (CharArray.undef_seg out (i + 1 ) (n + 1 ) )
+  **  (CharArray.full s_pre ((string_length (input)) + 1 ) (c_string (input)) )
+|--
+  EX (output: (@list Z)) ,
+  “ (n = (string_length (input))) ” 
+  &&  “ (out <> 0) ” 
+  &&  “ (0 <= i) ” 
+  &&  “ (i < n) ” 
+  &&  “ (0 <= (nletter + 1 )) ” 
+  &&  “ ((nletter + 1 ) <= (i + 1 )) ” 
+  &&  “ (0 <= (Znth i (c_string (input)) 0)) ” 
+  &&  “ ((Znth i (c_string (input)) 0) <= 127) ” 
+  &&  “ (flip_scan_state_z_161 input output (i + 1 ) (nletter + 1 ) ) ” 
+  &&  “ (valid_string input ) ” 
+  &&  “ (problem_161_pre_z input ) ” 
+  &&  “ (ascii_range_z input ) ” 
+  &&  “ ((string_length (input)) < INT_MAX) ”
+  &&  (store_string s_pre input )
+  **  (CharArray.full out (i + 1 ) output )
+  **  (CharArray.undef_seg out (i + 1 ) (n + 1 ) )
+) \/
+(
+forall (input: (@list Z)) (output_2: (@list Z)) (w: Z) (nletter: Z) (i: Z) (out: Z) (n: Z) (PreH1 : (0 <= ((string_length (input)) + 1 ))) (PreH2 : ((Znth i (c_string (input)) 0) < 97)) (PreH3 : ((Znth i (c_string (input)) 0) < 65)) (PreH4 : (i < n)) (PreH5 : (n = (string_length (input)))) (PreH6 : (out <> 0)) (PreH7 : (0 <= i)) (PreH8 : (i <= n)) (PreH9 : (0 <= nletter)) (PreH10 : (nletter <= i)) (PreH11 : (0 <= w)) (PreH12 : (w <= 127)) (PreH13 : (flip_scan_state_z_161 input output_2 i nletter )) (PreH14 : (valid_string input )) (PreH15 : (problem_161_pre_z input )) (PreH16 : (ascii_range_z input )) (PreH17 : ((string_length (input)) < INT_MAX)) ,
+  TT && emp 
+|--
+  “ (flip_scan_state_z_161 input (app (output_2) ((cons ((signed_last_nbits ((Znth i (c_string (input)) 0)) (8))) ((@nil Z))))) (i + 1 ) (nletter + 1 ) ) ” 
+  &&  “ (0 <= (Znth i (c_string (input)) 0)) ”
+  &&  emp
+).
+
+Definition solve_entail_wit_2_2_split_goal_1 := 
+forall (input: (@list Z)) (output_2: (@list Z)) (w: Z) (nletter: Z) (i: Z) (out: Z) (n: Z) (PreH1 : (0 <= ((string_length (input)) + 1 ))) (PreH2 : ((Znth i (c_string (input)) 0) < 97)) (PreH3 : ((Znth i (c_string (input)) 0) < 65)) (PreH4 : (i < n)) (PreH5 : (n = (string_length (input)))) (PreH6 : (out <> 0)) (PreH7 : (0 <= i)) (PreH8 : (i <= n)) (PreH9 : (0 <= nletter)) (PreH10 : (nletter <= i)) (PreH11 : (0 <= w)) (PreH12 : (w <= 127)) (PreH13 : (flip_scan_state_z_161 input output_2 i nletter )) (PreH14 : (valid_string input )) (PreH15 : (problem_161_pre_z input )) (PreH16 : (ascii_range_z input )) (PreH17 : ((string_length (input)) < INT_MAX)) ,
+  TT && emp 
+|--
+  “ (flip_scan_state_z_161 input (app (output_2) ((cons ((signed_last_nbits ((Znth i (c_string (input)) 0)) (8))) ((@nil Z))))) (i + 1 ) (nletter + 1 ) ) ”
+.
+
+Definition solve_entail_wit_2_2_split_goal_2 := 
+forall (input: (@list Z)) (output_2: (@list Z)) (w: Z) (nletter: Z) (i: Z) (out: Z) (n: Z) (PreH1 : (0 <= ((string_length (input)) + 1 ))) (PreH2 : ((Znth i (c_string (input)) 0) < 97)) (PreH3 : ((Znth i (c_string (input)) 0) < 65)) (PreH4 : (i < n)) (PreH5 : (n = (string_length (input)))) (PreH6 : (out <> 0)) (PreH7 : (0 <= i)) (PreH8 : (i <= n)) (PreH9 : (0 <= nletter)) (PreH10 : (nletter <= i)) (PreH11 : (0 <= w)) (PreH12 : (w <= 127)) (PreH13 : (flip_scan_state_z_161 input output_2 i nletter )) (PreH14 : (valid_string input )) (PreH15 : (problem_161_pre_z input )) (PreH16 : (ascii_range_z input )) (PreH17 : ((string_length (input)) < INT_MAX)) ,
+  TT && emp 
+|--
+  “ (0 <= (Znth i (c_string (input)) 0)) ”
+.
+
+Definition solve_entail_wit_2_3 := 
+(
+forall (s_pre: Z) (input: (@list Z)) (output_2: (@list Z)) (w: Z) (nletter: Z) (i: Z) (out: Z) (n: Z) (PreH1 : (0 <= ((string_length (input)) + 1 ))) (PreH2 : ((Znth i (c_string (input)) 0) < 97)) (PreH3 : ((Znth i (c_string (input)) 0) > 90)) (PreH4 : ((Znth i (c_string (input)) 0) >= 65)) (PreH5 : (i < n)) (PreH6 : (n = (string_length (input)))) (PreH7 : (out <> 0)) (PreH8 : (0 <= i)) (PreH9 : (i <= n)) (PreH10 : (0 <= nletter)) (PreH11 : (nletter <= i)) (PreH12 : (0 <= w)) (PreH13 : (w <= 127)) (PreH14 : (flip_scan_state_z_161 input output_2 i nletter )) (PreH15 : (valid_string input )) (PreH16 : (problem_161_pre_z input )) (PreH17 : (ascii_range_z input )) (PreH18 : ((string_length (input)) < INT_MAX)) ,
+  (CharArray.full out (i + 1 ) (app (output_2) ((cons ((Znth i (c_string (input)) 0)) ((@nil Z))))) )
+  **  (CharArray.undef_seg out (i + 1 ) (n + 1 ) )
+  **  (CharArray.full s_pre ((string_length (input)) + 1 ) (c_string (input)) )
+|--
+  EX (output: (@list Z)) ,
+  “ (n = (string_length (input))) ” 
+  &&  “ (out <> 0) ” 
+  &&  “ (0 <= i) ” 
+  &&  “ (i < n) ” 
+  &&  “ (0 <= (nletter + 1 )) ” 
+  &&  “ ((nletter + 1 ) <= (i + 1 )) ” 
+  &&  “ (0 <= (Znth i (c_string (input)) 0)) ” 
+  &&  “ ((Znth i (c_string (input)) 0) <= 127) ” 
+  &&  “ (flip_scan_state_z_161 input output (i + 1 ) (nletter + 1 ) ) ” 
+  &&  “ (valid_string input ) ” 
+  &&  “ (problem_161_pre_z input ) ” 
+  &&  “ (ascii_range_z input ) ” 
+  &&  “ ((string_length (input)) < INT_MAX) ”
+  &&  (store_string s_pre input )
+  **  (CharArray.full out (i + 1 ) output )
+  **  (CharArray.undef_seg out (i + 1 ) (n + 1 ) )
+) \/
+(
+forall (input: (@list Z)) (output_2: (@list Z)) (w: Z) (nletter: Z) (i: Z) (out: Z) (n: Z) (PreH1 : (0 <= ((string_length (input)) + 1 ))) (PreH2 : ((Znth i (c_string (input)) 0) < 97)) (PreH3 : ((Znth i (c_string (input)) 0) > 90)) (PreH4 : ((Znth i (c_string (input)) 0) >= 65)) (PreH5 : (i < n)) (PreH6 : (n = (string_length (input)))) (PreH7 : (out <> 0)) (PreH8 : (0 <= i)) (PreH9 : (i <= n)) (PreH10 : (0 <= nletter)) (PreH11 : (nletter <= i)) (PreH12 : (0 <= w)) (PreH13 : (w <= 127)) (PreH14 : (flip_scan_state_z_161 input output_2 i nletter )) (PreH15 : (valid_string input )) (PreH16 : (problem_161_pre_z input )) (PreH17 : (ascii_range_z input )) (PreH18 : ((string_length (input)) < INT_MAX)) ,
+  TT && emp 
+|--
+  “ (flip_scan_state_z_161 input (app (output_2) ((cons ((Znth i (c_string (input)) 0)) ((@nil Z))))) (i + 1 ) (nletter + 1 ) ) ”
+  &&  emp
+).
+
+Definition solve_entail_wit_2_3_split_goal_1 := 
+forall (input: (@list Z)) (output_2: (@list Z)) (w: Z) (nletter: Z) (i: Z) (out: Z) (n: Z) (PreH1 : (0 <= ((string_length (input)) + 1 ))) (PreH2 : ((Znth i (c_string (input)) 0) < 97)) (PreH3 : ((Znth i (c_string (input)) 0) > 90)) (PreH4 : ((Znth i (c_string (input)) 0) >= 65)) (PreH5 : (i < n)) (PreH6 : (n = (string_length (input)))) (PreH7 : (out <> 0)) (PreH8 : (0 <= i)) (PreH9 : (i <= n)) (PreH10 : (0 <= nletter)) (PreH11 : (nletter <= i)) (PreH12 : (0 <= w)) (PreH13 : (w <= 127)) (PreH14 : (flip_scan_state_z_161 input output_2 i nletter )) (PreH15 : (valid_string input )) (PreH16 : (problem_161_pre_z input )) (PreH17 : (ascii_range_z input )) (PreH18 : ((string_length (input)) < INT_MAX)) ,
+  TT && emp 
+|--
+  “ (flip_scan_state_z_161 input (app (output_2) ((cons ((Znth i (c_string (input)) 0)) ((@nil Z))))) (i + 1 ) (nletter + 1 ) ) ”
+.
+
+Definition solve_entail_wit_2_4 := 
+(
+forall (s_pre: Z) (input: (@list Z)) (output_2: (@list Z)) (w: Z) (nletter: Z) (i: Z) (out: Z) (n: Z) (PreH1 : (0 <= ((string_length (input)) + 1 ))) (PreH2 : ((Znth i (c_string (input)) 0) <= 122)) (PreH3 : ((Znth i (c_string (input)) 0) >= 97)) (PreH4 : ((Znth i (c_string (input)) 0) > 90)) (PreH5 : ((Znth i (c_string (input)) 0) >= 65)) (PreH6 : (i < n)) (PreH7 : (n = (string_length (input)))) (PreH8 : (out <> 0)) (PreH9 : (0 <= i)) (PreH10 : (i <= n)) (PreH11 : (0 <= nletter)) (PreH12 : (nletter <= i)) (PreH13 : (0 <= w)) (PreH14 : (w <= 127)) (PreH15 : (flip_scan_state_z_161 input output_2 i nletter )) (PreH16 : (valid_string input )) (PreH17 : (problem_161_pre_z input )) (PreH18 : (ascii_range_z input )) (PreH19 : ((string_length (input)) < INT_MAX)) ,
+  (CharArray.full out (i + 1 ) (app (output_2) ((cons (((Znth i (c_string (input)) 0) - 32 )) ((@nil Z))))) )
+  **  (CharArray.undef_seg out (i + 1 ) (n + 1 ) )
+  **  (CharArray.full s_pre ((string_length (input)) + 1 ) (c_string (input)) )
+|--
+  EX (output: (@list Z)) ,
+  “ (n = (string_length (input))) ” 
+  &&  “ (out <> 0) ” 
+  &&  “ (0 <= i) ” 
+  &&  “ (i < n) ” 
+  &&  “ (0 <= nletter) ” 
+  &&  “ (nletter <= (i + 1 )) ” 
+  &&  “ (0 <= ((Znth i (c_string (input)) 0) - 32 )) ” 
+  &&  “ (((Znth i (c_string (input)) 0) - 32 ) <= 127) ” 
+  &&  “ (flip_scan_state_z_161 input output (i + 1 ) nletter ) ” 
+  &&  “ (valid_string input ) ” 
+  &&  “ (problem_161_pre_z input ) ” 
+  &&  “ (ascii_range_z input ) ” 
+  &&  “ ((string_length (input)) < INT_MAX) ”
+  &&  (store_string s_pre input )
+  **  (CharArray.full out (i + 1 ) output )
+  **  (CharArray.undef_seg out (i + 1 ) (n + 1 ) )
+) \/
+(
+forall (input: (@list Z)) (output_2: (@list Z)) (w: Z) (nletter: Z) (i: Z) (out: Z) (n: Z) (PreH1 : (0 <= ((string_length (input)) + 1 ))) (PreH2 : ((Znth i (c_string (input)) 0) <= 122)) (PreH3 : ((Znth i (c_string (input)) 0) >= 97)) (PreH4 : ((Znth i (c_string (input)) 0) > 90)) (PreH5 : ((Znth i (c_string (input)) 0) >= 65)) (PreH6 : (i < n)) (PreH7 : (n = (string_length (input)))) (PreH8 : (out <> 0)) (PreH9 : (0 <= i)) (PreH10 : (i <= n)) (PreH11 : (0 <= nletter)) (PreH12 : (nletter <= i)) (PreH13 : (0 <= w)) (PreH14 : (w <= 127)) (PreH15 : (flip_scan_state_z_161 input output_2 i nletter )) (PreH16 : (valid_string input )) (PreH17 : (problem_161_pre_z input )) (PreH18 : (ascii_range_z input )) (PreH19 : ((string_length (input)) < INT_MAX)) ,
+  TT && emp 
+|--
+  “ (flip_scan_state_z_161 input (app (output_2) ((cons (((Znth i (c_string (input)) 0) - 32 )) ((@nil Z))))) (i + 1 ) nletter ) ”
+  &&  emp
+).
+
+Definition solve_entail_wit_2_4_split_goal_1 := 
+forall (input: (@list Z)) (output_2: (@list Z)) (w: Z) (nletter: Z) (i: Z) (out: Z) (n: Z) (PreH1 : (0 <= ((string_length (input)) + 1 ))) (PreH2 : ((Znth i (c_string (input)) 0) <= 122)) (PreH3 : ((Znth i (c_string (input)) 0) >= 97)) (PreH4 : ((Znth i (c_string (input)) 0) > 90)) (PreH5 : ((Znth i (c_string (input)) 0) >= 65)) (PreH6 : (i < n)) (PreH7 : (n = (string_length (input)))) (PreH8 : (out <> 0)) (PreH9 : (0 <= i)) (PreH10 : (i <= n)) (PreH11 : (0 <= nletter)) (PreH12 : (nletter <= i)) (PreH13 : (0 <= w)) (PreH14 : (w <= 127)) (PreH15 : (flip_scan_state_z_161 input output_2 i nletter )) (PreH16 : (valid_string input )) (PreH17 : (problem_161_pre_z input )) (PreH18 : (ascii_range_z input )) (PreH19 : ((string_length (input)) < INT_MAX)) ,
+  TT && emp 
+|--
+  “ (flip_scan_state_z_161 input (app (output_2) ((cons (((Znth i (c_string (input)) 0) - 32 )) ((@nil Z))))) (i + 1 ) nletter ) ”
+.
+
+Definition solve_entail_wit_2_5 := 
+(
+forall (s_pre: Z) (input: (@list Z)) (output_2: (@list Z)) (w: Z) (nletter: Z) (i: Z) (out: Z) (n: Z) (PreH1 : (0 <= ((string_length (input)) + 1 ))) (PreH2 : ((Znth i (c_string (input)) 0) <= 90)) (PreH3 : ((Znth i (c_string (input)) 0) >= 65)) (PreH4 : (i < n)) (PreH5 : (n = (string_length (input)))) (PreH6 : (out <> 0)) (PreH7 : (0 <= i)) (PreH8 : (i <= n)) (PreH9 : (0 <= nletter)) (PreH10 : (nletter <= i)) (PreH11 : (0 <= w)) (PreH12 : (w <= 127)) (PreH13 : (flip_scan_state_z_161 input output_2 i nletter )) (PreH14 : (valid_string input )) (PreH15 : (problem_161_pre_z input )) (PreH16 : (ascii_range_z input )) (PreH17 : ((string_length (input)) < INT_MAX)) ,
+  (CharArray.full out (i + 1 ) (app (output_2) ((cons (((Znth i (c_string (input)) 0) + 32 )) ((@nil Z))))) )
+  **  (CharArray.undef_seg out (i + 1 ) (n + 1 ) )
+  **  (CharArray.full s_pre ((string_length (input)) + 1 ) (c_string (input)) )
+|--
+  EX (output: (@list Z)) ,
+  “ (n = (string_length (input))) ” 
+  &&  “ (out <> 0) ” 
+  &&  “ (0 <= i) ” 
+  &&  “ (i < n) ” 
+  &&  “ (0 <= nletter) ” 
+  &&  “ (nletter <= (i + 1 )) ” 
+  &&  “ (0 <= ((Znth i (c_string (input)) 0) + 32 )) ” 
+  &&  “ (((Znth i (c_string (input)) 0) + 32 ) <= 127) ” 
+  &&  “ (flip_scan_state_z_161 input output (i + 1 ) nletter ) ” 
+  &&  “ (valid_string input ) ” 
+  &&  “ (problem_161_pre_z input ) ” 
+  &&  “ (ascii_range_z input ) ” 
+  &&  “ ((string_length (input)) < INT_MAX) ”
+  &&  (store_string s_pre input )
+  **  (CharArray.full out (i + 1 ) output )
+  **  (CharArray.undef_seg out (i + 1 ) (n + 1 ) )
+) \/
+(
+forall (input: (@list Z)) (output_2: (@list Z)) (w: Z) (nletter: Z) (i: Z) (out: Z) (n: Z) (PreH1 : (0 <= ((string_length (input)) + 1 ))) (PreH2 : ((Znth i (c_string (input)) 0) <= 90)) (PreH3 : ((Znth i (c_string (input)) 0) >= 65)) (PreH4 : (i < n)) (PreH5 : (n = (string_length (input)))) (PreH6 : (out <> 0)) (PreH7 : (0 <= i)) (PreH8 : (i <= n)) (PreH9 : (0 <= nletter)) (PreH10 : (nletter <= i)) (PreH11 : (0 <= w)) (PreH12 : (w <= 127)) (PreH13 : (flip_scan_state_z_161 input output_2 i nletter )) (PreH14 : (valid_string input )) (PreH15 : (problem_161_pre_z input )) (PreH16 : (ascii_range_z input )) (PreH17 : ((string_length (input)) < INT_MAX)) ,
+  TT && emp 
+|--
+  “ (flip_scan_state_z_161 input (app (output_2) ((cons (((Znth i (c_string (input)) 0) + 32 )) ((@nil Z))))) (i + 1 ) nletter ) ”
+  &&  emp
+).
+
+Definition solve_entail_wit_2_5_split_goal_1 := 
+forall (input: (@list Z)) (output_2: (@list Z)) (w: Z) (nletter: Z) (i: Z) (out: Z) (n: Z) (PreH1 : (0 <= ((string_length (input)) + 1 ))) (PreH2 : ((Znth i (c_string (input)) 0) <= 90)) (PreH3 : ((Znth i (c_string (input)) 0) >= 65)) (PreH4 : (i < n)) (PreH5 : (n = (string_length (input)))) (PreH6 : (out <> 0)) (PreH7 : (0 <= i)) (PreH8 : (i <= n)) (PreH9 : (0 <= nletter)) (PreH10 : (nletter <= i)) (PreH11 : (0 <= w)) (PreH12 : (w <= 127)) (PreH13 : (flip_scan_state_z_161 input output_2 i nletter )) (PreH14 : (valid_string input )) (PreH15 : (problem_161_pre_z input )) (PreH16 : (ascii_range_z input )) (PreH17 : ((string_length (input)) < INT_MAX)) ,
+  TT && emp 
+|--
+  “ (flip_scan_state_z_161 input (app (output_2) ((cons (((Znth i (c_string (input)) 0) + 32 )) ((@nil Z))))) (i + 1 ) nletter ) ”
+.
+
+Definition solve_entail_wit_3 := 
+forall (s_pre: Z) (input: (@list Z)) (output_2: (@list Z)) (n: Z) (out: Z) (i: Z) (nletter: Z) (w: Z) (PreH1 : (n = (string_length (input)))) (PreH2 : (out <> 0)) (PreH3 : (0 <= i)) (PreH4 : (i < n)) (PreH5 : (0 <= nletter)) (PreH6 : (nletter <= (i + 1 ))) (PreH7 : (0 <= w)) (PreH8 : (w <= 127)) (PreH9 : (flip_scan_state_z_161 input output_2 (i + 1 ) nletter )) (PreH10 : (valid_string input )) (PreH11 : (problem_161_pre_z input )) (PreH12 : (ascii_range_z input )) (PreH13 : ((string_length (input)) < INT_MAX)) ,
+  (store_string s_pre input )
+  **  (CharArray.full out (i + 1 ) output_2 )
+  **  (CharArray.undef_seg out (i + 1 ) (n + 1 ) )
+|--
+  EX (output: (@list Z)) ,
+  “ (n = (string_length (input))) ” 
+  &&  “ (out <> 0) ” 
+  &&  “ (0 <= (i + 1 )) ” 
+  &&  “ ((i + 1 ) <= n) ” 
+  &&  “ (0 <= nletter) ” 
+  &&  “ (nletter <= (i + 1 )) ” 
+  &&  “ (0 <= w) ” 
+  &&  “ (w <= 127) ” 
+  &&  “ (flip_scan_state_z_161 input output (i + 1 ) nletter ) ” 
+  &&  “ (valid_string input ) ” 
+  &&  “ (problem_161_pre_z input ) ” 
+  &&  “ (ascii_range_z input ) ” 
+  &&  “ ((string_length (input)) < INT_MAX) ”
+  &&  (store_string s_pre input )
+  **  (CharArray.full out (i + 1 ) output )
+  **  (CharArray.undef_seg out (i + 1 ) (n + 1 ) )
+.
+
+Definition solve_entail_wit_4 := 
+(
+forall (s_pre: Z) (input: (@list Z)) (output_2: (@list Z)) (w: Z) (nletter: Z) (i: Z) (out: Z) (n: Z) (PreH1 : (i >= n)) (PreH2 : (n = (string_length (input)))) (PreH3 : (out <> 0)) (PreH4 : (0 <= i)) (PreH5 : (i <= n)) (PreH6 : (0 <= nletter)) (PreH7 : (nletter <= i)) (PreH8 : (0 <= w)) (PreH9 : (w <= 127)) (PreH10 : (flip_scan_state_z_161 input output_2 i nletter )) (PreH11 : (valid_string input )) (PreH12 : (problem_161_pre_z input )) (PreH13 : (ascii_range_z input )) (PreH14 : ((string_length (input)) < INT_MAX)) ,
+  (store_string s_pre input )
+  **  (CharArray.full out i output_2 )
+  **  (CharArray.undef_seg out i (n + 1 ) )
+|--
+  EX (output: (@list Z)) ,
+  “ (n = (string_length (input))) ” 
+  &&  “ (i = n) ” 
+  &&  “ (out <> 0) ” 
+  &&  “ (0 <= nletter) ” 
+  &&  “ (nletter <= n) ” 
+  &&  “ (flip_scan_state_z_161 input output n nletter ) ” 
+  &&  “ (valid_string input ) ” 
+  &&  “ (problem_161_pre_z input ) ” 
+  &&  “ (ascii_range_z input ) ” 
+  &&  “ ((string_length (input)) < INT_MAX) ”
+  &&  (store_string s_pre input )
+  **  (CharArray.full out n output )
+  **  (CharArray.undef_seg out n (n + 1 ) )
+) \/
+(
+forall (input: (@list Z)) (output_2: (@list Z)) (w: Z) (nletter: Z) (i: Z) (out: Z) (n: Z) (PreH1 : (0 <= ((string_length (input)) + 1 ))) (PreH2 : (i >= n)) (PreH3 : (n = (string_length (input)))) (PreH4 : (out <> 0)) (PreH5 : (0 <= i)) (PreH6 : (i <= n)) (PreH7 : (0 <= nletter)) (PreH8 : (nletter <= i)) (PreH9 : (0 <= w)) (PreH10 : (w <= 127)) (PreH11 : (flip_scan_state_z_161 input output_2 i nletter )) (PreH12 : (valid_string input )) (PreH13 : (problem_161_pre_z input )) (PreH14 : (ascii_range_z input )) (PreH15 : ((string_length (input)) < INT_MAX)) ,
+  (CharArray.full out i output_2 )
+|--
+  EX (output: (@list Z)) ,
+  “ (n = (string_length (input))) ” 
+  &&  “ (i = n) ” 
+  &&  “ (out <> 0) ” 
+  &&  “ (0 <= nletter) ” 
+  &&  “ (nletter <= n) ” 
+  &&  “ (flip_scan_state_z_161 input output n nletter ) ” 
+  &&  “ (valid_string input ) ” 
+  &&  “ (problem_161_pre_z input ) ” 
+  &&  “ (ascii_range_z input ) ” 
+  &&  “ ((string_length (input)) < INT_MAX) ”
+  &&  (CharArray.full out n output )
+).
+
+Definition solve_entail_wit_5 := 
+(
+forall (s_pre: Z) (input: (@list Z)) (output_2: (@list Z)) (n: Z) (i: Z) (out: Z) (nletter: Z) (PreH1 : (nletter = n)) (PreH2 : (0 <= ((string_length (input)) + 1 ))) (PreH3 : (0 <= n)) (PreH4 : (n = (string_length (input)))) (PreH5 : (i = n)) (PreH6 : (out <> 0)) (PreH7 : (0 <= nletter)) (PreH8 : (nletter <= n)) (PreH9 : (flip_scan_state_z_161 input output_2 n nletter )) (PreH10 : (valid_string input )) (PreH11 : (problem_161_pre_z input )) (PreH12 : (ascii_range_z input )) (PreH13 : ((string_length (input)) < INT_MAX)) ,
+  (CharArray.full out (n + 1 ) (app (output_2) ((cons (0) ((@nil Z))))) )
+  **  (CharArray.undef_seg out (n + 1 ) (n + 1 ) )
+  **  (CharArray.full s_pre ((string_length (input)) + 1 ) (c_string (input)) )
+|--
+  EX (output: (@list Z)) ,
+  “ (n = (string_length (input))) ” 
+  &&  “ (i = n) ” 
+  &&  “ (out <> 0) ” 
+  &&  “ (nletter = n) ” 
+  &&  “ (no_letter_z_161 input ) ” 
+  &&  “ (flip_output_z_161 input output ) ” 
+  &&  “ (valid_string input ) ” 
+  &&  “ (valid_string output ) ” 
+  &&  “ (problem_161_pre_z input ) ” 
+  &&  “ (ascii_range_z input ) ” 
+  &&  “ ((string_length (input)) < INT_MAX) ”
+  &&  (store_string s_pre input )
+  **  (CharArray.full out (n + 1 ) (c_string (output)) )
+) \/
+(
+forall (input: (@list Z)) (output_2: (@list Z)) (n: Z) (i: Z) (out: Z) (nletter: Z) (PreH1 : (nletter = n)) (PreH2 : (0 <= ((string_length (input)) + 1 ))) (PreH3 : (0 <= n)) (PreH4 : (n = (string_length (input)))) (PreH5 : (i = n)) (PreH6 : (out <> 0)) (PreH7 : (0 <= nletter)) (PreH8 : (nletter <= n)) (PreH9 : (flip_scan_state_z_161 input output_2 n nletter )) (PreH10 : (valid_string input )) (PreH11 : (problem_161_pre_z input )) (PreH12 : (ascii_range_z input )) (PreH13 : ((string_length (input)) < INT_MAX)) ,
+  TT && emp 
+|--
+  EX (output: (@list Z)) ,
+  “ ((app (output_2) ((cons (0) ((@nil Z))))) = (c_string (output))) ” 
+  &&  “ (n = (string_length (input))) ” 
+  &&  “ (i = n) ” 
+  &&  “ (out <> 0) ” 
+  &&  “ (nletter = n) ” 
+  &&  “ (no_letter_z_161 input ) ” 
+  &&  “ (flip_output_z_161 input output ) ” 
+  &&  “ (valid_string input ) ” 
+  &&  “ (valid_string output ) ” 
+  &&  “ (problem_161_pre_z input ) ” 
+  &&  “ (ascii_range_z input ) ” 
+  &&  “ ((string_length (input)) < INT_MAX) ”
+  &&  emp
+).
+
+Definition solve_entail_wit_6 := 
+(
+forall (s_pre: Z) (input: (@list Z)) (output_2: (@list Z)) (n: Z) (i: Z) (out: Z) (nletter: Z) (retval: Z) (PreH1 : (retval <> 0)) (PreH2 : (retval <> 0)) (PreH3 : (0 <= ((string_length (input)) + 1 ))) (PreH4 : (0 <= (n + 1 ))) (PreH5 : (n = (string_length (input)))) (PreH6 : (i = n)) (PreH7 : (out <> 0)) (PreH8 : (nletter = n)) (PreH9 : (no_letter_z_161 input )) (PreH10 : (flip_output_z_161 input output_2 )) (PreH11 : (valid_string input )) (PreH12 : (valid_string output_2 )) (PreH13 : (problem_161_pre_z input )) (PreH14 : (ascii_range_z input )) (PreH15 : ((string_length (input)) < INT_MAX)) ,
+  (CharArray.undef_full retval (n + 1 ) )
+  **  (CharArray.full s_pre ((string_length (input)) + 1 ) (c_string (input)) )
+  **  (CharArray.full out (n + 1 ) (c_string (output_2)) )
+|--
+  EX (rev_output: (@list Z))  (output: (@list Z)) ,
+  “ (n = (string_length (input))) ” 
+  &&  “ (i = n) ” 
+  &&  “ (out <> 0) ” 
+  &&  “ (retval <> 0) ” 
+  &&  “ (nletter = n) ” 
+  &&  “ (0 <= 0) ” 
+  &&  “ (0 <= n) ” 
+  &&  “ (no_letter_z_161 input ) ” 
+  &&  “ (flip_output_z_161 input output ) ” 
+  &&  “ (reverse_scan_state_z_161 input rev_output 0 ) ” 
+  &&  “ (valid_string input ) ” 
+  &&  “ (valid_string output ) ” 
+  &&  “ (problem_161_pre_z input ) ” 
+  &&  “ (ascii_range_z input ) ” 
+  &&  “ ((string_length (input)) < INT_MAX) ”
+  &&  (store_string s_pre input )
+  **  (CharArray.full out (n + 1 ) (c_string (output)) )
+  **  (CharArray.full retval 0 rev_output )
+  **  (CharArray.undef_seg retval 0 (n + 1 ) )
+) \/
+(
+forall (input: (@list Z)) (output_2: (@list Z)) (n: Z) (i: Z) (out: Z) (nletter: Z) (retval: Z) (PreH1 : (retval <> 0)) (PreH2 : (retval <> 0)) (PreH3 : (0 <= ((string_length (input)) + 1 ))) (PreH4 : (0 <= (n + 1 ))) (PreH5 : (n = (string_length (input)))) (PreH6 : (i = n)) (PreH7 : (out <> 0)) (PreH8 : (nletter = n)) (PreH9 : (no_letter_z_161 input )) (PreH10 : (flip_output_z_161 input output_2 )) (PreH11 : (valid_string input )) (PreH12 : (valid_string output_2 )) (PreH13 : (problem_161_pre_z input )) (PreH14 : (ascii_range_z input )) (PreH15 : ((string_length (input)) < INT_MAX)) ,
+  (CharArray.undef_full retval (n + 1 ) )
+|--
+  EX (output: (@list Z)) ,
+  “ ((c_string (output_2)) = (c_string (output))) ” 
+  &&  “ (n = (string_length (input))) ” 
+  &&  “ (i = n) ” 
+  &&  “ (out <> 0) ” 
+  &&  “ (retval <> 0) ” 
+  &&  “ (nletter = n) ” 
+  &&  “ (0 <= 0) ” 
+  &&  “ (0 <= n) ” 
+  &&  “ (no_letter_z_161 input ) ” 
+  &&  “ (flip_output_z_161 input output ) ” 
+  &&  “ (reverse_scan_state_z_161 input (@nil Z) 0 ) ” 
+  &&  “ (valid_string input ) ” 
+  &&  “ (valid_string output ) ” 
+  &&  “ (problem_161_pre_z input ) ” 
+  &&  “ (ascii_range_z input ) ” 
+  &&  “ ((string_length (input)) < INT_MAX) ”
+  &&  (CharArray.undef_full retval (n + 1 ) )
+).
+
+Definition solve_entail_wit_7 := 
+(
+forall (s_pre: Z) (input: (@list Z)) (rev_output_2: (@list Z)) (output_2: (@list Z)) (j: Z) (nletter: Z) (p: Z) (out: Z) (i: Z) (n: Z) (PreH1 : (0 <= ((string_length (input)) + 1 ))) (PreH2 : (0 <= (n + 1 ))) (PreH3 : (j < n)) (PreH4 : (n = (string_length (input)))) (PreH5 : (i = n)) (PreH6 : (out <> 0)) (PreH7 : (p <> 0)) (PreH8 : (nletter = n)) (PreH9 : (0 <= j)) (PreH10 : (j <= n)) (PreH11 : (no_letter_z_161 input )) (PreH12 : (flip_output_z_161 input output_2 )) (PreH13 : (reverse_scan_state_z_161 input rev_output_2 j )) (PreH14 : (valid_string input )) (PreH15 : (valid_string output_2 )) (PreH16 : (problem_161_pre_z input )) (PreH17 : (ascii_range_z input )) (PreH18 : ((string_length (input)) < INT_MAX)) ,
+  (CharArray.full p (j + 1 ) (app (rev_output_2) ((cons ((Znth ((n - 1 ) - j ) (c_string (input)) 0)) ((@nil Z))))) )
+  **  (CharArray.undef_seg p (j + 1 ) (n + 1 ) )
+  **  (CharArray.full s_pre ((string_length (input)) + 1 ) (c_string (input)) )
+  **  (CharArray.full out (n + 1 ) (c_string (output_2)) )
+|--
+  EX (rev_output: (@list Z))  (output: (@list Z)) ,
+  “ (n = (string_length (input))) ” 
+  &&  “ (i = n) ” 
+  &&  “ (out <> 0) ” 
+  &&  “ (p <> 0) ” 
+  &&  “ (nletter = n) ” 
+  &&  “ (0 <= j) ” 
+  &&  “ (j < n) ” 
+  &&  “ (no_letter_z_161 input ) ” 
+  &&  “ (flip_output_z_161 input output ) ” 
+  &&  “ (reverse_scan_state_z_161 input rev_output (j + 1 ) ) ” 
+  &&  “ (valid_string input ) ” 
+  &&  “ (valid_string output ) ” 
+  &&  “ (problem_161_pre_z input ) ” 
+  &&  “ (ascii_range_z input ) ” 
+  &&  “ ((string_length (input)) < INT_MAX) ”
+  &&  (store_string s_pre input )
+  **  (CharArray.full out (n + 1 ) (c_string (output)) )
+  **  (CharArray.full p (j + 1 ) rev_output )
+  **  (CharArray.undef_seg p (j + 1 ) (n + 1 ) )
+) \/
+(
+forall (input: (@list Z)) (rev_output_2: (@list Z)) (output_2: (@list Z)) (j: Z) (nletter: Z) (p: Z) (out: Z) (i: Z) (n: Z) (PreH1 : (0 <= ((string_length (input)) + 1 ))) (PreH2 : (0 <= (n + 1 ))) (PreH3 : (j < n)) (PreH4 : (n = (string_length (input)))) (PreH5 : (i = n)) (PreH6 : (out <> 0)) (PreH7 : (p <> 0)) (PreH8 : (nletter = n)) (PreH9 : (0 <= j)) (PreH10 : (j <= n)) (PreH11 : (no_letter_z_161 input )) (PreH12 : (flip_output_z_161 input output_2 )) (PreH13 : (reverse_scan_state_z_161 input rev_output_2 j )) (PreH14 : (valid_string input )) (PreH15 : (valid_string output_2 )) (PreH16 : (problem_161_pre_z input )) (PreH17 : (ascii_range_z input )) (PreH18 : ((string_length (input)) < INT_MAX)) ,
+  TT && emp 
+|--
+  EX (output: (@list Z)) ,
+  “ ((c_string (output_2)) = (c_string (output))) ” 
+  &&  “ (n = (string_length (input))) ” 
+  &&  “ (i = n) ” 
+  &&  “ (out <> 0) ” 
+  &&  “ (p <> 0) ” 
+  &&  “ (nletter = n) ” 
+  &&  “ (0 <= j) ” 
+  &&  “ (j < n) ” 
+  &&  “ (no_letter_z_161 input ) ” 
+  &&  “ (flip_output_z_161 input output ) ” 
+  &&  “ (reverse_scan_state_z_161 input (app (rev_output_2) ((cons ((Znth ((n - 1 ) - j ) (c_string (input)) 0)) ((@nil Z))))) (j + 1 ) ) ” 
+  &&  “ (valid_string input ) ” 
+  &&  “ (valid_string output ) ” 
+  &&  “ (problem_161_pre_z input ) ” 
+  &&  “ (ascii_range_z input ) ” 
+  &&  “ ((string_length (input)) < INT_MAX) ”
+  &&  emp
+).
+
+Definition solve_entail_wit_8 := 
+forall (s_pre: Z) (input: (@list Z)) (output_2: (@list Z)) (rev_output_2: (@list Z)) (n: Z) (i: Z) (out: Z) (p: Z) (nletter: Z) (j: Z) (PreH1 : (n = (string_length (input)))) (PreH2 : (i = n)) (PreH3 : (out <> 0)) (PreH4 : (p <> 0)) (PreH5 : (nletter = n)) (PreH6 : (0 <= j)) (PreH7 : (j < n)) (PreH8 : (no_letter_z_161 input )) (PreH9 : (flip_output_z_161 input output_2 )) (PreH10 : (reverse_scan_state_z_161 input rev_output_2 (j + 1 ) )) (PreH11 : (valid_string input )) (PreH12 : (valid_string output_2 )) (PreH13 : (problem_161_pre_z input )) (PreH14 : (ascii_range_z input )) (PreH15 : ((string_length (input)) < INT_MAX)) ,
+  (store_string s_pre input )
+  **  (CharArray.full out (n + 1 ) (c_string (output_2)) )
+  **  (CharArray.full p (j + 1 ) rev_output_2 )
+  **  (CharArray.undef_seg p (j + 1 ) (n + 1 ) )
+|--
+  EX (rev_output: (@list Z))  (output: (@list Z)) ,
+  “ (n = (string_length (input))) ” 
+  &&  “ (i = n) ” 
+  &&  “ (out <> 0) ” 
+  &&  “ (p <> 0) ” 
+  &&  “ (nletter = n) ” 
+  &&  “ (0 <= (j + 1 )) ” 
+  &&  “ ((j + 1 ) <= n) ” 
+  &&  “ (no_letter_z_161 input ) ” 
+  &&  “ (flip_output_z_161 input output ) ” 
+  &&  “ (reverse_scan_state_z_161 input rev_output (j + 1 ) ) ” 
+  &&  “ (valid_string input ) ” 
+  &&  “ (valid_string output ) ” 
+  &&  “ (problem_161_pre_z input ) ” 
+  &&  “ (ascii_range_z input ) ” 
+  &&  “ ((string_length (input)) < INT_MAX) ”
+  &&  (store_string s_pre input )
+  **  (CharArray.full out (n + 1 ) (c_string (output)) )
+  **  (CharArray.full p (j + 1 ) rev_output )
+  **  (CharArray.undef_seg p (j + 1 ) (n + 1 ) )
+.
+
+Definition solve_entail_wit_9 := 
+(
+forall (s_pre: Z) (input: (@list Z)) (rev_output_2: (@list Z)) (output_2: (@list Z)) (j: Z) (nletter: Z) (p: Z) (out: Z) (i: Z) (n: Z) (PreH1 : (j >= n)) (PreH2 : (n = (string_length (input)))) (PreH3 : (i = n)) (PreH4 : (out <> 0)) (PreH5 : (p <> 0)) (PreH6 : (nletter = n)) (PreH7 : (0 <= j)) (PreH8 : (j <= n)) (PreH9 : (no_letter_z_161 input )) (PreH10 : (flip_output_z_161 input output_2 )) (PreH11 : (reverse_scan_state_z_161 input rev_output_2 j )) (PreH12 : (valid_string input )) (PreH13 : (valid_string output_2 )) (PreH14 : (problem_161_pre_z input )) (PreH15 : (ascii_range_z input )) (PreH16 : ((string_length (input)) < INT_MAX)) ,
+  (store_string s_pre input )
+  **  (CharArray.full out (n + 1 ) (c_string (output_2)) )
+  **  (CharArray.full p j rev_output_2 )
+  **  (CharArray.undef_seg p j (n + 1 ) )
+|--
+  EX (rev_output: (@list Z))  (output: (@list Z)) ,
+  “ (n = (string_length (input))) ” 
+  &&  “ (i = n) ” 
+  &&  “ (j = n) ” 
+  &&  “ (out <> 0) ” 
+  &&  “ (p <> 0) ” 
+  &&  “ (nletter = n) ” 
+  &&  “ (no_letter_z_161 input ) ” 
+  &&  “ (flip_output_z_161 input output ) ” 
+  &&  “ (reverse_output_z_161 input rev_output ) ” 
+  &&  “ (valid_string input ) ” 
+  &&  “ (valid_string output ) ” 
+  &&  “ (valid_string rev_output ) ” 
+  &&  “ (problem_161_pre_z input ) ” 
+  &&  “ (problem_161_spec_z input rev_output ) ” 
+  &&  “ (ascii_range_z input ) ” 
+  &&  “ ((string_length (input)) < INT_MAX) ”
+  &&  (store_string s_pre input )
+  **  (CharArray.full out (n + 1 ) (c_string (output)) )
+  **  (CharArray.full p n rev_output )
+  **  (CharArray.undef_seg p n (n + 1 ) )
+) \/
+(
+forall (input: (@list Z)) (rev_output_2: (@list Z)) (output_2: (@list Z)) (j: Z) (nletter: Z) (p: Z) (out: Z) (i: Z) (n: Z) (PreH1 : (0 <= ((string_length (input)) + 1 ))) (PreH2 : (j >= n)) (PreH3 : (n = (string_length (input)))) (PreH4 : (i = n)) (PreH5 : (out <> 0)) (PreH6 : (p <> 0)) (PreH7 : (nletter = n)) (PreH8 : (0 <= j)) (PreH9 : (j <= n)) (PreH10 : (no_letter_z_161 input )) (PreH11 : (flip_output_z_161 input output_2 )) (PreH12 : (reverse_scan_state_z_161 input rev_output_2 j )) (PreH13 : (valid_string input )) (PreH14 : (valid_string output_2 )) (PreH15 : (problem_161_pre_z input )) (PreH16 : (ascii_range_z input )) (PreH17 : ((string_length (input)) < INT_MAX)) ,
+  (CharArray.full p j rev_output_2 )
+|--
+  EX (rev_output: (@list Z))  (output: (@list Z)) ,
+  “ ((c_string (output_2)) = (c_string (output))) ” 
+  &&  “ (n = (string_length (input))) ” 
+  &&  “ (i = n) ” 
+  &&  “ (j = n) ” 
+  &&  “ (out <> 0) ” 
+  &&  “ (p <> 0) ” 
+  &&  “ (nletter = n) ” 
+  &&  “ (no_letter_z_161 input ) ” 
+  &&  “ (flip_output_z_161 input output ) ” 
+  &&  “ (reverse_output_z_161 input rev_output ) ” 
+  &&  “ (valid_string input ) ” 
+  &&  “ (valid_string output ) ” 
+  &&  “ (valid_string rev_output ) ” 
+  &&  “ (problem_161_pre_z input ) ” 
+  &&  “ (problem_161_spec_z input rev_output ) ” 
+  &&  “ (ascii_range_z input ) ” 
+  &&  “ ((string_length (input)) < INT_MAX) ”
+  &&  (CharArray.full p n rev_output )
+).
+
+Definition solve_entail_wit_10 := 
+(
+forall (s_pre: Z) (input: (@list Z)) (output_2: (@list Z)) (n: Z) (i: Z) (out: Z) (nletter: Z) (PreH1 : (nletter <> n)) (PreH2 : (0 <= ((string_length (input)) + 1 ))) (PreH3 : (0 <= n)) (PreH4 : (n = (string_length (input)))) (PreH5 : (i = n)) (PreH6 : (out <> 0)) (PreH7 : (0 <= nletter)) (PreH8 : (nletter <= n)) (PreH9 : (flip_scan_state_z_161 input output_2 n nletter )) (PreH10 : (valid_string input )) (PreH11 : (problem_161_pre_z input )) (PreH12 : (ascii_range_z input )) (PreH13 : ((string_length (input)) < INT_MAX)) ,
+  (CharArray.full out (n + 1 ) (app (output_2) ((cons (0) ((@nil Z))))) )
+  **  (CharArray.undef_seg out (n + 1 ) (n + 1 ) )
+  **  (CharArray.full s_pre ((string_length (input)) + 1 ) (c_string (input)) )
+|--
+  EX (output: (@list Z)) ,
+  “ (n = (string_length (input))) ” 
+  &&  “ (i = n) ” 
+  &&  “ (out <> 0) ” 
+  &&  “ (nletter <> n) ” 
+  &&  “ (has_letter_z_161 input ) ” 
+  &&  “ (flip_output_z_161 input output ) ” 
+  &&  “ (valid_string input ) ” 
+  &&  “ (valid_string output ) ” 
+  &&  “ (problem_161_pre_z input ) ” 
+  &&  “ (problem_161_spec_z input output ) ” 
+  &&  “ (ascii_range_z input ) ” 
+  &&  “ ((string_length (input)) < INT_MAX) ”
+  &&  (store_string s_pre input )
+  **  (CharArray.full out (n + 1 ) (c_string (output)) )
+) \/
+(
+forall (input: (@list Z)) (output_2: (@list Z)) (n: Z) (i: Z) (out: Z) (nletter: Z) (PreH1 : (nletter <> n)) (PreH2 : (0 <= ((string_length (input)) + 1 ))) (PreH3 : (0 <= n)) (PreH4 : (n = (string_length (input)))) (PreH5 : (i = n)) (PreH6 : (out <> 0)) (PreH7 : (0 <= nletter)) (PreH8 : (nletter <= n)) (PreH9 : (flip_scan_state_z_161 input output_2 n nletter )) (PreH10 : (valid_string input )) (PreH11 : (problem_161_pre_z input )) (PreH12 : (ascii_range_z input )) (PreH13 : ((string_length (input)) < INT_MAX)) ,
+  TT && emp 
+|--
+  EX (output: (@list Z)) ,
+  “ ((app (output_2) ((cons (0) ((@nil Z))))) = (c_string (output))) ” 
+  &&  “ (n = (string_length (input))) ” 
+  &&  “ (i = n) ” 
+  &&  “ (out <> 0) ” 
+  &&  “ (nletter <> n) ” 
+  &&  “ (has_letter_z_161 input ) ” 
+  &&  “ (flip_output_z_161 input output ) ” 
+  &&  “ (valid_string input ) ” 
+  &&  “ (valid_string output ) ” 
+  &&  “ (problem_161_pre_z input ) ” 
+  &&  “ (problem_161_spec_z input output ) ” 
+  &&  “ (ascii_range_z input ) ” 
+  &&  “ ((string_length (input)) < INT_MAX) ”
+  &&  emp
+).
+
+Definition solve_return_wit_1 := 
+(
+forall (s_pre: Z) (input: (@list Z)) (output_2: (@list Z)) (n: Z) (i: Z) (out: Z) (nletter: Z) (PreH1 : (n = (string_length (input)))) (PreH2 : (i = n)) (PreH3 : (out <> 0)) (PreH4 : (nletter <> n)) (PreH5 : (has_letter_z_161 input )) (PreH6 : (flip_output_z_161 input output_2 )) (PreH7 : (valid_string input )) (PreH8 : (valid_string output_2 )) (PreH9 : (problem_161_pre_z input )) (PreH10 : (problem_161_spec_z input output_2 )) (PreH11 : (ascii_range_z input )) (PreH12 : ((string_length (input)) < INT_MAX)) ,
+  (store_string s_pre input )
+  **  (CharArray.full out (n + 1 ) (c_string (output_2)) )
+|--
+  EX (output: (@list Z)) ,
+  “ (problem_161_spec_z input output ) ” 
+  &&  “ (valid_string output ) ”
+  &&  (store_string s_pre input )
+  **  (store_string out output )
+) \/
+(
+forall (input: (@list Z)) (output_2: (@list Z)) (n: Z) (i: Z) (out: Z) (nletter: Z) (PreH1 : (0 <= ((string_length (input)) + 1 ))) (PreH2 : (0 <= (n + 1 ))) (PreH3 : (n = (string_length (input)))) (PreH4 : (i = n)) (PreH5 : (out <> 0)) (PreH6 : (nletter <> n)) (PreH7 : (has_letter_z_161 input )) (PreH8 : (flip_output_z_161 input output_2 )) (PreH9 : (valid_string input )) (PreH10 : (valid_string output_2 )) (PreH11 : (problem_161_pre_z input )) (PreH12 : (problem_161_spec_z input output_2 )) (PreH13 : (ascii_range_z input )) (PreH14 : ((string_length (input)) < INT_MAX)) ,
+  (CharArray.full out (n + 1 ) (c_string (output_2)) )
+|--
+  EX (output: (@list Z)) ,
+  “ (problem_161_spec_z input output ) ” 
+  &&  “ (valid_string output ) ”
+  &&  (CharArray.full out ((string_length (output)) + 1 ) (c_string (output)) )
+).
+
+Definition solve_return_wit_2 := 
+(
+forall (s_pre: Z) (input: (@list Z)) (output_2: (@list Z)) (rev_output: (@list Z)) (n: Z) (i: Z) (j: Z) (out: Z) (p: Z) (nletter: Z) (PreH1 : (0 <= ((string_length (input)) + 1 ))) (PreH2 : (0 <= n)) (PreH3 : (0 <= (n + 1 ))) (PreH4 : (n = (string_length (input)))) (PreH5 : (i = n)) (PreH6 : (j = n)) (PreH7 : (out <> 0)) (PreH8 : (p <> 0)) (PreH9 : (nletter = n)) (PreH10 : (no_letter_z_161 input )) (PreH11 : (flip_output_z_161 input output_2 )) (PreH12 : (reverse_output_z_161 input rev_output )) (PreH13 : (valid_string input )) (PreH14 : (valid_string output_2 )) (PreH15 : (valid_string rev_output )) (PreH16 : (problem_161_pre_z input )) (PreH17 : (problem_161_spec_z input rev_output )) (PreH18 : (ascii_range_z input )) (PreH19 : ((string_length (input)) < INT_MAX)) ,
+  (CharArray.full p (n + 1 ) (app (rev_output) ((cons (0) ((@nil Z))))) )
+  **  (CharArray.full s_pre ((string_length (input)) + 1 ) (c_string (input)) )
+|--
+  EX (output: (@list Z)) ,
+  “ (problem_161_spec_z input output ) ” 
+  &&  “ (valid_string output ) ”
+  &&  (store_string s_pre input )
+  **  (store_string p output )
+) \/
+(
+forall (input: (@list Z)) (output_2: (@list Z)) (rev_output: (@list Z)) (n: Z) (i: Z) (j: Z) (out: Z) (p: Z) (nletter: Z) (PreH1 : (0 <= ((string_length (input)) + 1 ))) (PreH2 : (0 <= n)) (PreH3 : (0 <= (n + 1 ))) (PreH4 : (n = (string_length (input)))) (PreH5 : (i = n)) (PreH6 : (j = n)) (PreH7 : (out <> 0)) (PreH8 : (p <> 0)) (PreH9 : (nletter = n)) (PreH10 : (no_letter_z_161 input )) (PreH11 : (flip_output_z_161 input output_2 )) (PreH12 : (reverse_output_z_161 input rev_output )) (PreH13 : (valid_string input )) (PreH14 : (valid_string output_2 )) (PreH15 : (valid_string rev_output )) (PreH16 : (problem_161_pre_z input )) (PreH17 : (problem_161_spec_z input rev_output )) (PreH18 : (ascii_range_z input )) (PreH19 : ((string_length (input)) < INT_MAX)) ,
+  (CharArray.full p (n + 1 ) (app (rev_output) ((cons (0) ((@nil Z))))) )
+|--
+  EX (output: (@list Z)) ,
+  “ (problem_161_spec_z input output ) ” 
+  &&  “ (valid_string output ) ”
+  &&  (CharArray.full p ((string_length (output)) + 1 ) (c_string (output)) )
+).
+
+Definition solve_partial_solve_wit_1_pure := 
+forall (s_pre: Z) (input: (@list Z)) (PreH1 : (valid_string input )) (PreH2 : (problem_161_pre_z input )) (PreH3 : (ascii_range_z input )) (PreH4 : ((string_length (input)) < INT_MAX)) ,
+  ((( &( "n" ) )) # Int  |->_)
+  **  ((( &( "s" ) )) # Ptr  |-> s_pre)
+  **  (store_string s_pre input )
+|--
+  “ (valid_string input ) ” 
+  &&  “ ((string_length (input)) < INT_MAX) ”
+.
+
+Definition solve_partial_solve_wit_1_aux := 
+forall (s_pre: Z) (input: (@list Z)) (PreH1 : (valid_string input )) (PreH2 : (problem_161_pre_z input )) (PreH3 : (ascii_range_z input )) (PreH4 : ((string_length (input)) < INT_MAX)) ,
+  (store_string s_pre input )
+|--
+  “ (valid_string input ) ” 
+  &&  “ ((string_length (input)) < INT_MAX) ” 
+  &&  “ (0 <= ((string_length (input)) + 1 )) ” 
+  &&  “ (valid_string input ) ” 
+  &&  “ (problem_161_pre_z input ) ” 
+  &&  “ (ascii_range_z input ) ” 
+  &&  “ ((string_length (input)) < INT_MAX) ”
+  &&  (store_string s_pre input )
+.
+
+Definition solve_partial_solve_wit_1 := solve_partial_solve_wit_1_pure -> solve_partial_solve_wit_1_aux.
+
+Definition solve_partial_solve_wit_2_pure := 
+(
+forall (s_pre: Z) (input: (@list Z)) (retval: Z) (PreH1 : (retval = (string_length (input)))) (PreH2 : (0 <= ((string_length (input)) + 1 ))) (PreH3 : (valid_string input )) (PreH4 : (problem_161_pre_z input )) (PreH5 : (ascii_range_z input )) (PreH6 : ((string_length (input)) < INT_MAX)) ,
+  ((( &( "out" ) )) # Ptr  |->_)
+  **  ((( &( "nletter" ) )) # Int  |-> 0)
+  **  (store_string s_pre input )
+  **  ((( &( "n" ) )) # Int  |-> retval)
+  **  ((( &( "s" ) )) # Ptr  |-> s_pre)
+|--
+  “ ((retval + 1 ) <= INT_MAX) ” 
+  &&  “ ((retval + 1 ) > 0) ”
+) \/
+(
+forall (s_pre: Z) (input: (@list Z)) (retval: Z) (PreH1 : (retval <= INT_MAX)) (PreH2 : (0 <= INT_MAX)) (PreH3 : (retval >= INT_MIN)) (PreH4 : (0 >= INT_MIN)) (PreH5 : (retval = (string_length (input)))) (PreH6 : (0 <= ((string_length (input)) + 1 ))) (PreH7 : (valid_string input )) (PreH8 : (problem_161_pre_z input )) (PreH9 : (ascii_range_z input )) (PreH10 : ((string_length (input)) < INT_MAX)) ,
+  (CharArray.full s_pre ((string_length (input)) + 1 ) (c_string (input)) )
+  **  ((( &( "out" ) )) # Ptr  |->_)
+  **  ((( &( "nletter" ) )) # Int  |-> 0)
+  **  ((( &( "n" ) )) # Int  |-> retval)
+  **  ((( &( "s" ) )) # Ptr  |-> s_pre)
+|--
+  “ ((retval + 1 ) > 0) ”
+).
+
+Definition solve_partial_solve_wit_2_pure_split_goal_1 := 
+forall (s_pre: Z) (input: (@list Z)) (retval: Z) (PreH1 : (retval <= INT_MAX)) (PreH2 : (0 <= INT_MAX)) (PreH3 : (retval >= INT_MIN)) (PreH4 : (0 >= INT_MIN)) (PreH5 : (retval = (string_length (input)))) (PreH6 : (0 <= ((string_length (input)) + 1 ))) (PreH7 : (valid_string input )) (PreH8 : (problem_161_pre_z input )) (PreH9 : (ascii_range_z input )) (PreH10 : ((string_length (input)) < INT_MAX)) ,
+  (CharArray.full s_pre ((string_length (input)) + 1 ) (c_string (input)) )
+  **  ((( &( "out" ) )) # Ptr  |->_)
+  **  ((( &( "nletter" ) )) # Int  |-> 0)
+  **  ((( &( "n" ) )) # Int  |-> retval)
+  **  ((( &( "s" ) )) # Ptr  |-> s_pre)
+|--
+  “ ((retval + 1 ) > 0) ”
+.
+
+Definition solve_partial_solve_wit_2_aux := 
+forall (s_pre: Z) (input: (@list Z)) (retval: Z) (PreH1 : (retval = (string_length (input)))) (PreH2 : (0 <= ((string_length (input)) + 1 ))) (PreH3 : (valid_string input )) (PreH4 : (problem_161_pre_z input )) (PreH5 : (ascii_range_z input )) (PreH6 : ((string_length (input)) < INT_MAX)) ,
+  (store_string s_pre input )
+|--
+  “ ((retval + 1 ) <= INT_MAX) ” 
+  &&  “ ((retval + 1 ) > 0) ” 
+  &&  “ (retval = (string_length (input))) ” 
+  &&  “ (0 <= ((string_length (input)) + 1 )) ” 
+  &&  “ (valid_string input ) ” 
+  &&  “ (problem_161_pre_z input ) ” 
+  &&  “ (ascii_range_z input ) ” 
+  &&  “ ((string_length (input)) < INT_MAX) ”
+  &&  (CharArray.full s_pre ((string_length (input)) + 1 ) (c_string (input)) )
+.
+
+Definition solve_partial_solve_wit_2 := solve_partial_solve_wit_2_pure -> solve_partial_solve_wit_2_aux.
+
+Definition solve_partial_solve_wit_3 := 
+forall (s_pre: Z) (input: (@list Z)) (output: (@list Z)) (w: Z) (nletter: Z) (i: Z) (out: Z) (n: Z) (PreH1 : ((Znth i (c_string (input)) 0) <= 90)) (PreH2 : ((Znth i (c_string (input)) 0) >= 65)) (PreH3 : (i < n)) (PreH4 : (n = (string_length (input)))) (PreH5 : (out <> 0)) (PreH6 : (0 <= i)) (PreH7 : (i <= n)) (PreH8 : (0 <= nletter)) (PreH9 : (nletter <= i)) (PreH10 : (0 <= w)) (PreH11 : (w <= 127)) (PreH12 : (flip_scan_state_z_161 input output i nletter )) (PreH13 : (valid_string input )) (PreH14 : (problem_161_pre_z input )) (PreH15 : (ascii_range_z input )) (PreH16 : ((string_length (input)) < INT_MAX)) ,
+  (store_string s_pre input )
+  **  (CharArray.full out i output )
+  **  (CharArray.undef_seg out i (n + 1 ) )
+|--
+  “ (0 <= ((string_length (input)) + 1 )) ” 
+  &&  “ ((Znth i (c_string (input)) 0) <= 90) ” 
+  &&  “ ((Znth i (c_string (input)) 0) >= 65) ” 
+  &&  “ (i < n) ” 
+  &&  “ (n = (string_length (input))) ” 
+  &&  “ (out <> 0) ” 
+  &&  “ (0 <= i) ” 
+  &&  “ (i <= n) ” 
+  &&  “ (0 <= nletter) ” 
+  &&  “ (nletter <= i) ” 
+  &&  “ (0 <= w) ” 
+  &&  “ (w <= 127) ” 
+  &&  “ (flip_scan_state_z_161 input output i nletter ) ” 
+  &&  “ (valid_string input ) ” 
+  &&  “ (problem_161_pre_z input ) ” 
+  &&  “ (ascii_range_z input ) ” 
+  &&  “ ((string_length (input)) < INT_MAX) ”
+  &&  (((out + (i * sizeof(CHAR) ) )) # Char  |->_)
+  **  (CharArray.full s_pre ((string_length (input)) + 1 ) (c_string (input)) )
+  **  (CharArray.undef_missing_i out i i (n + 1 ) )
+  **  (CharArray.full out i output )
+.
+
+Definition solve_partial_solve_wit_4 := 
+forall (s_pre: Z) (input: (@list Z)) (output: (@list Z)) (w: Z) (nletter: Z) (i: Z) (out: Z) (n: Z) (PreH1 : ((Znth i (c_string (input)) 0) <= 122)) (PreH2 : ((Znth i (c_string (input)) 0) >= 97)) (PreH3 : ((Znth i (c_string (input)) 0) > 90)) (PreH4 : ((Znth i (c_string (input)) 0) >= 65)) (PreH5 : (i < n)) (PreH6 : (n = (string_length (input)))) (PreH7 : (out <> 0)) (PreH8 : (0 <= i)) (PreH9 : (i <= n)) (PreH10 : (0 <= nletter)) (PreH11 : (nletter <= i)) (PreH12 : (0 <= w)) (PreH13 : (w <= 127)) (PreH14 : (flip_scan_state_z_161 input output i nletter )) (PreH15 : (valid_string input )) (PreH16 : (problem_161_pre_z input )) (PreH17 : (ascii_range_z input )) (PreH18 : ((string_length (input)) < INT_MAX)) ,
+  (store_string s_pre input )
+  **  (CharArray.full out i output )
+  **  (CharArray.undef_seg out i (n + 1 ) )
+|--
+  “ (0 <= ((string_length (input)) + 1 )) ” 
+  &&  “ ((Znth i (c_string (input)) 0) <= 122) ” 
+  &&  “ ((Znth i (c_string (input)) 0) >= 97) ” 
+  &&  “ ((Znth i (c_string (input)) 0) > 90) ” 
+  &&  “ ((Znth i (c_string (input)) 0) >= 65) ” 
+  &&  “ (i < n) ” 
+  &&  “ (n = (string_length (input))) ” 
+  &&  “ (out <> 0) ” 
+  &&  “ (0 <= i) ” 
+  &&  “ (i <= n) ” 
+  &&  “ (0 <= nletter) ” 
+  &&  “ (nletter <= i) ” 
+  &&  “ (0 <= w) ” 
+  &&  “ (w <= 127) ” 
+  &&  “ (flip_scan_state_z_161 input output i nletter ) ” 
+  &&  “ (valid_string input ) ” 
+  &&  “ (problem_161_pre_z input ) ” 
+  &&  “ (ascii_range_z input ) ” 
+  &&  “ ((string_length (input)) < INT_MAX) ”
+  &&  (((out + (i * sizeof(CHAR) ) )) # Char  |->_)
+  **  (CharArray.full s_pre ((string_length (input)) + 1 ) (c_string (input)) )
+  **  (CharArray.undef_missing_i out i i (n + 1 ) )
+  **  (CharArray.full out i output )
+.
+
+Definition solve_partial_solve_wit_5 := 
+forall (s_pre: Z) (input: (@list Z)) (output: (@list Z)) (w: Z) (nletter: Z) (i: Z) (out: Z) (n: Z) (PreH1 : ((Znth i (c_string (input)) 0) < 97)) (PreH2 : ((Znth i (c_string (input)) 0) > 90)) (PreH3 : ((Znth i (c_string (input)) 0) >= 65)) (PreH4 : (i < n)) (PreH5 : (n = (string_length (input)))) (PreH6 : (out <> 0)) (PreH7 : (0 <= i)) (PreH8 : (i <= n)) (PreH9 : (0 <= nletter)) (PreH10 : (nletter <= i)) (PreH11 : (0 <= w)) (PreH12 : (w <= 127)) (PreH13 : (flip_scan_state_z_161 input output i nletter )) (PreH14 : (valid_string input )) (PreH15 : (problem_161_pre_z input )) (PreH16 : (ascii_range_z input )) (PreH17 : ((string_length (input)) < INT_MAX)) ,
+  (store_string s_pre input )
+  **  (CharArray.full out i output )
+  **  (CharArray.undef_seg out i (n + 1 ) )
+|--
+  “ (0 <= ((string_length (input)) + 1 )) ” 
+  &&  “ ((Znth i (c_string (input)) 0) < 97) ” 
+  &&  “ ((Znth i (c_string (input)) 0) > 90) ” 
+  &&  “ ((Znth i (c_string (input)) 0) >= 65) ” 
+  &&  “ (i < n) ” 
+  &&  “ (n = (string_length (input))) ” 
+  &&  “ (out <> 0) ” 
+  &&  “ (0 <= i) ” 
+  &&  “ (i <= n) ” 
+  &&  “ (0 <= nletter) ” 
+  &&  “ (nletter <= i) ” 
+  &&  “ (0 <= w) ” 
+  &&  “ (w <= 127) ” 
+  &&  “ (flip_scan_state_z_161 input output i nletter ) ” 
+  &&  “ (valid_string input ) ” 
+  &&  “ (problem_161_pre_z input ) ” 
+  &&  “ (ascii_range_z input ) ” 
+  &&  “ ((string_length (input)) < INT_MAX) ”
+  &&  (((out + (i * sizeof(CHAR) ) )) # Char  |->_)
+  **  (CharArray.full s_pre ((string_length (input)) + 1 ) (c_string (input)) )
+  **  (CharArray.undef_missing_i out i i (n + 1 ) )
+  **  (CharArray.full out i output )
+.
+
+Definition solve_partial_solve_wit_6 := 
+forall (s_pre: Z) (input: (@list Z)) (output: (@list Z)) (w: Z) (nletter: Z) (i: Z) (out: Z) (n: Z) (PreH1 : ((Znth i (c_string (input)) 0) < 97)) (PreH2 : ((Znth i (c_string (input)) 0) < 65)) (PreH3 : (i < n)) (PreH4 : (n = (string_length (input)))) (PreH5 : (out <> 0)) (PreH6 : (0 <= i)) (PreH7 : (i <= n)) (PreH8 : (0 <= nletter)) (PreH9 : (nletter <= i)) (PreH10 : (0 <= w)) (PreH11 : (w <= 127)) (PreH12 : (flip_scan_state_z_161 input output i nletter )) (PreH13 : (valid_string input )) (PreH14 : (problem_161_pre_z input )) (PreH15 : (ascii_range_z input )) (PreH16 : ((string_length (input)) < INT_MAX)) ,
+  (store_string s_pre input )
+  **  (CharArray.full out i output )
+  **  (CharArray.undef_seg out i (n + 1 ) )
+|--
+  “ (0 <= ((string_length (input)) + 1 )) ” 
+  &&  “ ((Znth i (c_string (input)) 0) < 97) ” 
+  &&  “ ((Znth i (c_string (input)) 0) < 65) ” 
+  &&  “ (i < n) ” 
+  &&  “ (n = (string_length (input))) ” 
+  &&  “ (out <> 0) ” 
+  &&  “ (0 <= i) ” 
+  &&  “ (i <= n) ” 
+  &&  “ (0 <= nletter) ” 
+  &&  “ (nletter <= i) ” 
+  &&  “ (0 <= w) ” 
+  &&  “ (w <= 127) ” 
+  &&  “ (flip_scan_state_z_161 input output i nletter ) ” 
+  &&  “ (valid_string input ) ” 
+  &&  “ (problem_161_pre_z input ) ” 
+  &&  “ (ascii_range_z input ) ” 
+  &&  “ ((string_length (input)) < INT_MAX) ”
+  &&  (((out + (i * sizeof(CHAR) ) )) # Char  |->_)
+  **  (CharArray.full s_pre ((string_length (input)) + 1 ) (c_string (input)) )
+  **  (CharArray.undef_missing_i out i i (n + 1 ) )
+  **  (CharArray.full out i output )
+.
+
+Definition solve_partial_solve_wit_7 := 
+forall (s_pre: Z) (input: (@list Z)) (output: (@list Z)) (w: Z) (nletter: Z) (i: Z) (out: Z) (n: Z) (PreH1 : ((Znth i (c_string (input)) 0) > 122)) (PreH2 : ((Znth i (c_string (input)) 0) >= 97)) (PreH3 : ((Znth i (c_string (input)) 0) > 90)) (PreH4 : ((Znth i (c_string (input)) 0) >= 65)) (PreH5 : (i < n)) (PreH6 : (n = (string_length (input)))) (PreH7 : (out <> 0)) (PreH8 : (0 <= i)) (PreH9 : (i <= n)) (PreH10 : (0 <= nletter)) (PreH11 : (nletter <= i)) (PreH12 : (0 <= w)) (PreH13 : (w <= 127)) (PreH14 : (flip_scan_state_z_161 input output i nletter )) (PreH15 : (valid_string input )) (PreH16 : (problem_161_pre_z input )) (PreH17 : (ascii_range_z input )) (PreH18 : ((string_length (input)) < INT_MAX)) ,
+  (store_string s_pre input )
+  **  (CharArray.full out i output )
+  **  (CharArray.undef_seg out i (n + 1 ) )
+|--
+  “ (0 <= ((string_length (input)) + 1 )) ” 
+  &&  “ ((Znth i (c_string (input)) 0) > 122) ” 
+  &&  “ ((Znth i (c_string (input)) 0) >= 97) ” 
+  &&  “ ((Znth i (c_string (input)) 0) > 90) ” 
+  &&  “ ((Znth i (c_string (input)) 0) >= 65) ” 
+  &&  “ (i < n) ” 
+  &&  “ (n = (string_length (input))) ” 
+  &&  “ (out <> 0) ” 
+  &&  “ (0 <= i) ” 
+  &&  “ (i <= n) ” 
+  &&  “ (0 <= nletter) ” 
+  &&  “ (nletter <= i) ” 
+  &&  “ (0 <= w) ” 
+  &&  “ (w <= 127) ” 
+  &&  “ (flip_scan_state_z_161 input output i nletter ) ” 
+  &&  “ (valid_string input ) ” 
+  &&  “ (problem_161_pre_z input ) ” 
+  &&  “ (ascii_range_z input ) ” 
+  &&  “ ((string_length (input)) < INT_MAX) ”
+  &&  (((out + (i * sizeof(CHAR) ) )) # Char  |->_)
+  **  (CharArray.full s_pre ((string_length (input)) + 1 ) (c_string (input)) )
+  **  (CharArray.undef_missing_i out i i (n + 1 ) )
+  **  (CharArray.full out i output )
+.
+
+Definition solve_partial_solve_wit_8 := 
+forall (s_pre: Z) (input: (@list Z)) (output: (@list Z)) (n: Z) (i: Z) (out: Z) (nletter: Z) (PreH1 : (n = (string_length (input)))) (PreH2 : (i = n)) (PreH3 : (out <> 0)) (PreH4 : (0 <= nletter)) (PreH5 : (nletter <= n)) (PreH6 : (flip_scan_state_z_161 input output n nletter )) (PreH7 : (valid_string input )) (PreH8 : (problem_161_pre_z input )) (PreH9 : (ascii_range_z input )) (PreH10 : ((string_length (input)) < INT_MAX)) ,
+  (store_string s_pre input )
+  **  (CharArray.full out n output )
+  **  (CharArray.undef_seg out n (n + 1 ) )
+|--
+  “ (0 <= ((string_length (input)) + 1 )) ” 
+  &&  “ (0 <= n) ” 
+  &&  “ (n = (string_length (input))) ” 
+  &&  “ (i = n) ” 
+  &&  “ (out <> 0) ” 
+  &&  “ (0 <= nletter) ” 
+  &&  “ (nletter <= n) ” 
+  &&  “ (flip_scan_state_z_161 input output n nletter ) ” 
+  &&  “ (valid_string input ) ” 
+  &&  “ (problem_161_pre_z input ) ” 
+  &&  “ (ascii_range_z input ) ” 
+  &&  “ ((string_length (input)) < INT_MAX) ”
+  &&  (((out + (n * sizeof(CHAR) ) )) # Char  |->_)
+  **  (CharArray.full s_pre ((string_length (input)) + 1 ) (c_string (input)) )
+  **  (CharArray.undef_missing_i out n n (n + 1 ) )
+  **  (CharArray.full out n output )
+.
+
+Definition solve_partial_solve_wit_9_pure := 
+(
+forall (s_pre: Z) (input: (@list Z)) (output: (@list Z)) (n: Z) (i: Z) (out: Z) (nletter: Z) (w: Z) (PreH1 : (n = (string_length (input)))) (PreH2 : (i = n)) (PreH3 : (out <> 0)) (PreH4 : (nletter = n)) (PreH5 : (no_letter_z_161 input )) (PreH6 : (flip_output_z_161 input output )) (PreH7 : (valid_string input )) (PreH8 : (valid_string output )) (PreH9 : (problem_161_pre_z input )) (PreH10 : (ascii_range_z input )) (PreH11 : ((string_length (input)) < INT_MAX)) ,
+  ((( &( "p" ) )) # Ptr  |->_)
+  **  ((( &( "s" ) )) # Ptr  |-> s_pre)
+  **  ((( &( "n" ) )) # Int  |-> n)
+  **  ((( &( "i" ) )) # Int  |-> i)
+  **  ((( &( "out" ) )) # Ptr  |-> out)
+  **  ((( &( "nletter" ) )) # Int  |-> nletter)
+  **  ((( &( "w" ) )) # Int  |-> w)
+  **  (store_string s_pre input )
+  **  (CharArray.full out (n + 1 ) (c_string (output)) )
+|--
+  “ ((n + 1 ) <= INT_MAX) ” 
+  &&  “ ((n + 1 ) > 0) ”
+) \/
+(
+forall (s_pre: Z) (input: (@list Z)) (output: (@list Z)) (n: Z) (i: Z) (out: Z) (nletter: Z) (w: Z) (PreH1 : (w <= INT_MAX)) (PreH2 : (nletter <= INT_MAX)) (PreH3 : (i <= INT_MAX)) (PreH4 : (n <= INT_MAX)) (PreH5 : (w >= INT_MIN)) (PreH6 : (nletter >= INT_MIN)) (PreH7 : (i >= INT_MIN)) (PreH8 : (n >= INT_MIN)) (PreH9 : (0 <= ((string_length (input)) + 1 ))) (PreH10 : (0 <= (n + 1 ))) (PreH11 : (n = (string_length (input)))) (PreH12 : (i = n)) (PreH13 : (out <> 0)) (PreH14 : (nletter = n)) (PreH15 : (no_letter_z_161 input )) (PreH16 : (flip_output_z_161 input output )) (PreH17 : (valid_string input )) (PreH18 : (valid_string output )) (PreH19 : (problem_161_pre_z input )) (PreH20 : (ascii_range_z input )) (PreH21 : ((string_length (input)) < INT_MAX)) ,
+  (CharArray.full s_pre ((string_length (input)) + 1 ) (c_string (input)) )
+  **  ((( &( "p" ) )) # Ptr  |->_)
+  **  ((( &( "s" ) )) # Ptr  |-> s_pre)
+  **  ((( &( "n" ) )) # Int  |-> n)
+  **  ((( &( "i" ) )) # Int  |-> i)
+  **  ((( &( "out" ) )) # Ptr  |-> out)
+  **  ((( &( "nletter" ) )) # Int  |-> nletter)
+  **  ((( &( "w" ) )) # Int  |-> w)
+  **  (CharArray.full out (n + 1 ) (c_string (output)) )
+|--
+  “ ((n + 1 ) > 0) ”
+).
+
+Definition solve_partial_solve_wit_9_pure_split_goal_1 := 
+forall (s_pre: Z) (input: (@list Z)) (output: (@list Z)) (n: Z) (i: Z) (out: Z) (nletter: Z) (w: Z) (PreH1 : (w <= INT_MAX)) (PreH2 : (nletter <= INT_MAX)) (PreH3 : (i <= INT_MAX)) (PreH4 : (n <= INT_MAX)) (PreH5 : (w >= INT_MIN)) (PreH6 : (nletter >= INT_MIN)) (PreH7 : (i >= INT_MIN)) (PreH8 : (n >= INT_MIN)) (PreH9 : (0 <= ((string_length (input)) + 1 ))) (PreH10 : (0 <= (n + 1 ))) (PreH11 : (n = (string_length (input)))) (PreH12 : (i = n)) (PreH13 : (out <> 0)) (PreH14 : (nletter = n)) (PreH15 : (no_letter_z_161 input )) (PreH16 : (flip_output_z_161 input output )) (PreH17 : (valid_string input )) (PreH18 : (valid_string output )) (PreH19 : (problem_161_pre_z input )) (PreH20 : (ascii_range_z input )) (PreH21 : ((string_length (input)) < INT_MAX)) ,
+  (CharArray.full s_pre ((string_length (input)) + 1 ) (c_string (input)) )
+  **  ((( &( "p" ) )) # Ptr  |->_)
+  **  ((( &( "s" ) )) # Ptr  |-> s_pre)
+  **  ((( &( "n" ) )) # Int  |-> n)
+  **  ((( &( "i" ) )) # Int  |-> i)
+  **  ((( &( "out" ) )) # Ptr  |-> out)
+  **  ((( &( "nletter" ) )) # Int  |-> nletter)
+  **  ((( &( "w" ) )) # Int  |-> w)
+  **  (CharArray.full out (n + 1 ) (c_string (output)) )
+|--
+  “ ((n + 1 ) > 0) ”
+.
+
+Definition solve_partial_solve_wit_9_aux := 
+forall (s_pre: Z) (input: (@list Z)) (output: (@list Z)) (n: Z) (i: Z) (out: Z) (nletter: Z) (PreH1 : (n = (string_length (input)))) (PreH2 : (i = n)) (PreH3 : (out <> 0)) (PreH4 : (nletter = n)) (PreH5 : (no_letter_z_161 input )) (PreH6 : (flip_output_z_161 input output )) (PreH7 : (valid_string input )) (PreH8 : (valid_string output )) (PreH9 : (problem_161_pre_z input )) (PreH10 : (ascii_range_z input )) (PreH11 : ((string_length (input)) < INT_MAX)) ,
+  (store_string s_pre input )
+  **  (CharArray.full out (n + 1 ) (c_string (output)) )
+|--
+  “ ((n + 1 ) <= INT_MAX) ” 
+  &&  “ ((n + 1 ) > 0) ” 
+  &&  “ (0 <= ((string_length (input)) + 1 )) ” 
+  &&  “ (0 <= (n + 1 )) ” 
+  &&  “ (n = (string_length (input))) ” 
+  &&  “ (i = n) ” 
+  &&  “ (out <> 0) ” 
+  &&  “ (nletter = n) ” 
+  &&  “ (no_letter_z_161 input ) ” 
+  &&  “ (flip_output_z_161 input output ) ” 
+  &&  “ (valid_string input ) ” 
+  &&  “ (valid_string output ) ” 
+  &&  “ (problem_161_pre_z input ) ” 
+  &&  “ (ascii_range_z input ) ” 
+  &&  “ ((string_length (input)) < INT_MAX) ”
+  &&  (CharArray.full s_pre ((string_length (input)) + 1 ) (c_string (input)) )
+  **  (CharArray.full out (n + 1 ) (c_string (output)) )
+.
+
+Definition solve_partial_solve_wit_9 := solve_partial_solve_wit_9_pure -> solve_partial_solve_wit_9_aux.
+
+Definition solve_partial_solve_wit_10 := 
+forall (s_pre: Z) (input: (@list Z)) (rev_output: (@list Z)) (output: (@list Z)) (j: Z) (nletter: Z) (p: Z) (out: Z) (i: Z) (n: Z) (PreH1 : (j < n)) (PreH2 : (n = (string_length (input)))) (PreH3 : (i = n)) (PreH4 : (out <> 0)) (PreH5 : (p <> 0)) (PreH6 : (nletter = n)) (PreH7 : (0 <= j)) (PreH8 : (j <= n)) (PreH9 : (no_letter_z_161 input )) (PreH10 : (flip_output_z_161 input output )) (PreH11 : (reverse_scan_state_z_161 input rev_output j )) (PreH12 : (valid_string input )) (PreH13 : (valid_string output )) (PreH14 : (problem_161_pre_z input )) (PreH15 : (ascii_range_z input )) (PreH16 : ((string_length (input)) < INT_MAX)) ,
+  (store_string s_pre input )
+  **  (CharArray.full out (n + 1 ) (c_string (output)) )
+  **  (CharArray.full p j rev_output )
+  **  (CharArray.undef_seg p j (n + 1 ) )
+|--
+  “ (0 <= ((string_length (input)) + 1 )) ” 
+  &&  “ (0 <= (n + 1 )) ” 
+  &&  “ (j < n) ” 
+  &&  “ (n = (string_length (input))) ” 
+  &&  “ (i = n) ” 
+  &&  “ (out <> 0) ” 
+  &&  “ (p <> 0) ” 
+  &&  “ (nletter = n) ” 
+  &&  “ (0 <= j) ” 
+  &&  “ (j <= n) ” 
+  &&  “ (no_letter_z_161 input ) ” 
+  &&  “ (flip_output_z_161 input output ) ” 
+  &&  “ (reverse_scan_state_z_161 input rev_output j ) ” 
+  &&  “ (valid_string input ) ” 
+  &&  “ (valid_string output ) ” 
+  &&  “ (problem_161_pre_z input ) ” 
+  &&  “ (ascii_range_z input ) ” 
+  &&  “ ((string_length (input)) < INT_MAX) ”
+  &&  (((p + (j * sizeof(CHAR) ) )) # Char  |->_)
+  **  (CharArray.full s_pre ((string_length (input)) + 1 ) (c_string (input)) )
+  **  (CharArray.undef_missing_i p j j (n + 1 ) )
+  **  (CharArray.full out (n + 1 ) (c_string (output)) )
+  **  (CharArray.full p j rev_output )
+.
+
+Definition solve_partial_solve_wit_11 := 
+forall (s_pre: Z) (input: (@list Z)) (output: (@list Z)) (rev_output: (@list Z)) (n: Z) (i: Z) (j: Z) (out: Z) (p: Z) (nletter: Z) (PreH1 : (n = (string_length (input)))) (PreH2 : (i = n)) (PreH3 : (j = n)) (PreH4 : (out <> 0)) (PreH5 : (p <> 0)) (PreH6 : (nletter = n)) (PreH7 : (no_letter_z_161 input )) (PreH8 : (flip_output_z_161 input output )) (PreH9 : (reverse_output_z_161 input rev_output )) (PreH10 : (valid_string input )) (PreH11 : (valid_string output )) (PreH12 : (valid_string rev_output )) (PreH13 : (problem_161_pre_z input )) (PreH14 : (problem_161_spec_z input rev_output )) (PreH15 : (ascii_range_z input )) (PreH16 : ((string_length (input)) < INT_MAX)) ,
+  (store_string s_pre input )
+  **  (CharArray.full out (n + 1 ) (c_string (output)) )
+  **  (CharArray.full p n rev_output )
+  **  (CharArray.undef_seg p n (n + 1 ) )
+|--
+  “ (0 <= ((string_length (input)) + 1 )) ” 
+  &&  “ (0 <= n) ” 
+  &&  “ (0 <= (n + 1 )) ” 
+  &&  “ (n = (string_length (input))) ” 
+  &&  “ (i = n) ” 
+  &&  “ (j = n) ” 
+  &&  “ (out <> 0) ” 
+  &&  “ (p <> 0) ” 
+  &&  “ (nletter = n) ” 
+  &&  “ (no_letter_z_161 input ) ” 
+  &&  “ (flip_output_z_161 input output ) ” 
+  &&  “ (reverse_output_z_161 input rev_output ) ” 
+  &&  “ (valid_string input ) ” 
+  &&  “ (valid_string output ) ” 
+  &&  “ (valid_string rev_output ) ” 
+  &&  “ (problem_161_pre_z input ) ” 
+  &&  “ (problem_161_spec_z input rev_output ) ” 
+  &&  “ (ascii_range_z input ) ” 
+  &&  “ ((string_length (input)) < INT_MAX) ”
+  &&  (((p + (n * sizeof(CHAR) ) )) # Char  |->_)
+  **  (CharArray.full s_pre ((string_length (input)) + 1 ) (c_string (input)) )
+  **  (CharArray.undef_missing_i p n n (n + 1 ) )
+  **  (CharArray.full out (n + 1 ) (c_string (output)) )
+  **  (CharArray.full p n rev_output )
+.
+
+Definition solve_partial_solve_wit_12_pure := 
+(
+forall (s_pre: Z) (input: (@list Z)) (output: (@list Z)) (rev_output: (@list Z)) (n: Z) (i: Z) (j: Z) (out: Z) (p: Z) (nletter: Z) (w: Z) (PreH1 : (0 <= ((string_length (input)) + 1 ))) (PreH2 : (0 <= n)) (PreH3 : (0 <= (n + 1 ))) (PreH4 : (n = (string_length (input)))) (PreH5 : (i = n)) (PreH6 : (j = n)) (PreH7 : (out <> 0)) (PreH8 : (p <> 0)) (PreH9 : (nletter = n)) (PreH10 : (no_letter_z_161 input )) (PreH11 : (flip_output_z_161 input output )) (PreH12 : (reverse_output_z_161 input rev_output )) (PreH13 : (valid_string input )) (PreH14 : (valid_string output )) (PreH15 : (valid_string rev_output )) (PreH16 : (problem_161_pre_z input )) (PreH17 : (problem_161_spec_z input rev_output )) (PreH18 : (ascii_range_z input )) (PreH19 : ((string_length (input)) < INT_MAX)) ,
+  (CharArray.full p (n + 1 ) (app (rev_output) ((cons (0) ((@nil Z))))) )
+  **  (CharArray.undef_seg p (n + 1 ) (n + 1 ) )
+  **  (CharArray.full s_pre ((string_length (input)) + 1 ) (c_string (input)) )
+  **  ((( &( "s" ) )) # Ptr  |-> s_pre)
+  **  ((( &( "n" ) )) # Int  |-> n)
+  **  ((( &( "i" ) )) # Int  |-> i)
+  **  ((( &( "j" ) )) # Int  |-> j)
+  **  ((( &( "out" ) )) # Ptr  |-> out)
+  **  ((( &( "p" ) )) # Ptr  |-> p)
+  **  ((( &( "nletter" ) )) # Int  |-> nletter)
+  **  ((( &( "w" ) )) # Int  |-> w)
+  **  (CharArray.full out (n + 1 ) (c_string (output)) )
+|--
+  “ (out <> 0) ” 
+  &&  “ (0 < (n + 1 )) ” 
+  &&  “ ((n + 1 ) <= INT_MAX) ” 
+  &&  “ ((Zlength ((c_string (output)))) = (n + 1 )) ”
+) \/
+(
+forall (s_pre: Z) (input: (@list Z)) (output: (@list Z)) (rev_output: (@list Z)) (n: Z) (i: Z) (j: Z) (out: Z) (p: Z) (nletter: Z) (w: Z) (PreH1 : (w <= INT_MAX)) (PreH2 : (nletter <= INT_MAX)) (PreH3 : (j <= INT_MAX)) (PreH4 : (i <= INT_MAX)) (PreH5 : (n <= INT_MAX)) (PreH6 : (w >= INT_MIN)) (PreH7 : (nletter >= INT_MIN)) (PreH8 : (j >= INT_MIN)) (PreH9 : (i >= INT_MIN)) (PreH10 : (n >= INT_MIN)) (PreH11 : (0 <= ((string_length (input)) + 1 ))) (PreH12 : (0 <= n)) (PreH13 : (0 <= (n + 1 ))) (PreH14 : (n = (string_length (input)))) (PreH15 : (i = n)) (PreH16 : (j = n)) (PreH17 : (out <> 0)) (PreH18 : (p <> 0)) (PreH19 : (nletter = n)) (PreH20 : (no_letter_z_161 input )) (PreH21 : (flip_output_z_161 input output )) (PreH22 : (reverse_output_z_161 input rev_output )) (PreH23 : (valid_string input )) (PreH24 : (valid_string output )) (PreH25 : (valid_string rev_output )) (PreH26 : (problem_161_pre_z input )) (PreH27 : (problem_161_spec_z input rev_output )) (PreH28 : (ascii_range_z input )) (PreH29 : ((string_length (input)) < INT_MAX)) ,
+  (CharArray.full p (n + 1 ) (app (rev_output) ((cons (0) ((@nil Z))))) )
+  **  (CharArray.full s_pre ((string_length (input)) + 1 ) (c_string (input)) )
+  **  ((( &( "s" ) )) # Ptr  |-> s_pre)
+  **  ((( &( "n" ) )) # Int  |-> n)
+  **  ((( &( "i" ) )) # Int  |-> i)
+  **  ((( &( "j" ) )) # Int  |-> j)
+  **  ((( &( "out" ) )) # Ptr  |-> out)
+  **  ((( &( "p" ) )) # Ptr  |-> p)
+  **  ((( &( "nletter" ) )) # Int  |-> nletter)
+  **  ((( &( "w" ) )) # Int  |-> w)
+  **  (CharArray.full out (n + 1 ) (c_string (output)) )
+|--
+  “ ((Zlength ((c_string (output)))) = (n + 1 )) ”
+).
+
+Definition solve_partial_solve_wit_12_pure_split_goal_1 := 
+forall (s_pre: Z) (input: (@list Z)) (output: (@list Z)) (rev_output: (@list Z)) (n: Z) (i: Z) (j: Z) (out: Z) (p: Z) (nletter: Z) (w: Z) (PreH1 : (w <= INT_MAX)) (PreH2 : (nletter <= INT_MAX)) (PreH3 : (j <= INT_MAX)) (PreH4 : (i <= INT_MAX)) (PreH5 : (n <= INT_MAX)) (PreH6 : (w >= INT_MIN)) (PreH7 : (nletter >= INT_MIN)) (PreH8 : (j >= INT_MIN)) (PreH9 : (i >= INT_MIN)) (PreH10 : (n >= INT_MIN)) (PreH11 : (0 <= ((string_length (input)) + 1 ))) (PreH12 : (0 <= n)) (PreH13 : (0 <= (n + 1 ))) (PreH14 : (n = (string_length (input)))) (PreH15 : (i = n)) (PreH16 : (j = n)) (PreH17 : (out <> 0)) (PreH18 : (p <> 0)) (PreH19 : (nletter = n)) (PreH20 : (no_letter_z_161 input )) (PreH21 : (flip_output_z_161 input output )) (PreH22 : (reverse_output_z_161 input rev_output )) (PreH23 : (valid_string input )) (PreH24 : (valid_string output )) (PreH25 : (valid_string rev_output )) (PreH26 : (problem_161_pre_z input )) (PreH27 : (problem_161_spec_z input rev_output )) (PreH28 : (ascii_range_z input )) (PreH29 : ((string_length (input)) < INT_MAX)) ,
+  (CharArray.full p (n + 1 ) (app (rev_output) ((cons (0) ((@nil Z))))) )
+  **  (CharArray.full s_pre ((string_length (input)) + 1 ) (c_string (input)) )
+  **  ((( &( "s" ) )) # Ptr  |-> s_pre)
+  **  ((( &( "n" ) )) # Int  |-> n)
+  **  ((( &( "i" ) )) # Int  |-> i)
+  **  ((( &( "j" ) )) # Int  |-> j)
+  **  ((( &( "out" ) )) # Ptr  |-> out)
+  **  ((( &( "p" ) )) # Ptr  |-> p)
+  **  ((( &( "nletter" ) )) # Int  |-> nletter)
+  **  ((( &( "w" ) )) # Int  |-> w)
+  **  (CharArray.full out (n + 1 ) (c_string (output)) )
+|--
+  “ ((Zlength ((c_string (output)))) = (n + 1 )) ”
+.
+
+Definition solve_partial_solve_wit_12_aux := 
+forall (s_pre: Z) (input: (@list Z)) (output: (@list Z)) (rev_output: (@list Z)) (n: Z) (i: Z) (j: Z) (out: Z) (p: Z) (nletter: Z) (PreH1 : (0 <= ((string_length (input)) + 1 ))) (PreH2 : (0 <= n)) (PreH3 : (0 <= (n + 1 ))) (PreH4 : (n = (string_length (input)))) (PreH5 : (i = n)) (PreH6 : (j = n)) (PreH7 : (out <> 0)) (PreH8 : (p <> 0)) (PreH9 : (nletter = n)) (PreH10 : (no_letter_z_161 input )) (PreH11 : (flip_output_z_161 input output )) (PreH12 : (reverse_output_z_161 input rev_output )) (PreH13 : (valid_string input )) (PreH14 : (valid_string output )) (PreH15 : (valid_string rev_output )) (PreH16 : (problem_161_pre_z input )) (PreH17 : (problem_161_spec_z input rev_output )) (PreH18 : (ascii_range_z input )) (PreH19 : ((string_length (input)) < INT_MAX)) ,
+  (CharArray.full p (n + 1 ) (app (rev_output) ((cons (0) ((@nil Z))))) )
+  **  (CharArray.undef_seg p (n + 1 ) (n + 1 ) )
+  **  (CharArray.full s_pre ((string_length (input)) + 1 ) (c_string (input)) )
+  **  (CharArray.full out (n + 1 ) (c_string (output)) )
+|--
+  “ (out <> 0) ” 
+  &&  “ (0 < (n + 1 )) ” 
+  &&  “ ((n + 1 ) <= INT_MAX) ” 
+  &&  “ ((Zlength ((c_string (output)))) = (n + 1 )) ” 
+  &&  “ (0 <= ((string_length (input)) + 1 )) ” 
+  &&  “ (0 <= n) ” 
+  &&  “ (0 <= (n + 1 )) ” 
+  &&  “ (n = (string_length (input))) ” 
+  &&  “ (i = n) ” 
+  &&  “ (j = n) ” 
+  &&  “ (out <> 0) ” 
+  &&  “ (p <> 0) ” 
+  &&  “ (nletter = n) ” 
+  &&  “ (no_letter_z_161 input ) ” 
+  &&  “ (flip_output_z_161 input output ) ” 
+  &&  “ (reverse_output_z_161 input rev_output ) ” 
+  &&  “ (valid_string input ) ” 
+  &&  “ (valid_string output ) ” 
+  &&  “ (valid_string rev_output ) ” 
+  &&  “ (problem_161_pre_z input ) ” 
+  &&  “ (problem_161_spec_z input rev_output ) ” 
+  &&  “ (ascii_range_z input ) ” 
+  &&  “ ((string_length (input)) < INT_MAX) ”
+  &&  (CharArray.full out (n + 1 ) (c_string (output)) )
+  **  (CharArray.full p (n + 1 ) (app (rev_output) ((cons (0) ((@nil Z))))) )
+  **  (CharArray.full s_pre ((string_length (input)) + 1 ) (c_string (input)) )
+.
+
+Definition solve_partial_solve_wit_12 := solve_partial_solve_wit_12_pure -> solve_partial_solve_wit_12_aux.
+
+Module Type VC_Correct.
+
+Include char_array_Strategy_Correct.
+Include string_Strategy_Correct.
+
+Axiom proof_of_solve_safety_wit_1 : solve_safety_wit_1.
+Axiom proof_of_solve_safety_wit_2 : solve_safety_wit_2.
+Axiom proof_of_solve_safety_wit_3 : solve_safety_wit_3.
+Axiom proof_of_solve_safety_wit_4 : solve_safety_wit_4.
+Axiom proof_of_solve_safety_wit_5 : solve_safety_wit_5.
+Axiom proof_of_solve_safety_wit_6 : solve_safety_wit_6.
+Axiom proof_of_solve_safety_wit_7 : solve_safety_wit_7.
+Axiom proof_of_solve_safety_wit_8 : solve_safety_wit_8.
+Axiom proof_of_solve_safety_wit_9 : solve_safety_wit_9.
+Axiom proof_of_solve_safety_wit_10 : solve_safety_wit_10.
+Axiom proof_of_solve_safety_wit_11 : solve_safety_wit_11.
+Axiom proof_of_solve_safety_wit_12 : solve_safety_wit_12.
+Axiom proof_of_solve_safety_wit_13 : solve_safety_wit_13.
+Axiom proof_of_solve_safety_wit_14 : solve_safety_wit_14.
+Axiom proof_of_solve_safety_wit_15 : solve_safety_wit_15.
+Axiom proof_of_solve_safety_wit_16 : solve_safety_wit_16.
+Axiom proof_of_solve_safety_wit_17 : solve_safety_wit_17.
+Axiom proof_of_solve_safety_wit_18 : solve_safety_wit_18.
+Axiom proof_of_solve_safety_wit_19 : solve_safety_wit_19.
+Axiom proof_of_solve_safety_wit_20 : solve_safety_wit_20.
+Axiom proof_of_solve_safety_wit_21 : solve_safety_wit_21.
+Axiom proof_of_solve_safety_wit_22 : solve_safety_wit_22.
+Axiom proof_of_solve_safety_wit_23 : solve_safety_wit_23.
+Axiom proof_of_solve_safety_wit_24 : solve_safety_wit_24.
+Axiom proof_of_solve_safety_wit_25 : solve_safety_wit_25.
+Axiom proof_of_solve_safety_wit_26 : solve_safety_wit_26.
+Axiom proof_of_solve_safety_wit_27 : solve_safety_wit_27.
+Axiom proof_of_solve_safety_wit_28 : solve_safety_wit_28.
+Axiom proof_of_solve_safety_wit_29 : solve_safety_wit_29.
+Axiom proof_of_solve_safety_wit_30 : solve_safety_wit_30.
+Axiom proof_of_solve_safety_wit_31 : solve_safety_wit_31.
+Axiom proof_of_solve_safety_wit_32 : solve_safety_wit_32.
+Axiom proof_of_solve_safety_wit_33 : solve_safety_wit_33.
+Axiom proof_of_solve_safety_wit_34 : solve_safety_wit_34.
+Axiom proof_of_solve_safety_wit_35 : solve_safety_wit_35.
+Axiom proof_of_solve_safety_wit_36 : solve_safety_wit_36.
+Axiom proof_of_solve_safety_wit_37 : solve_safety_wit_37.
+Axiom proof_of_solve_entail_wit_1 : solve_entail_wit_1.
+Axiom proof_of_solve_entail_wit_2_1 : solve_entail_wit_2_1.
+Axiom proof_of_solve_entail_wit_2_2 : solve_entail_wit_2_2.
+Axiom proof_of_solve_entail_wit_2_3 : solve_entail_wit_2_3.
+Axiom proof_of_solve_entail_wit_2_4 : solve_entail_wit_2_4.
+Axiom proof_of_solve_entail_wit_2_5 : solve_entail_wit_2_5.
+Axiom proof_of_solve_entail_wit_3 : solve_entail_wit_3.
+Axiom proof_of_solve_entail_wit_4 : solve_entail_wit_4.
+Axiom proof_of_solve_entail_wit_5 : solve_entail_wit_5.
+Axiom proof_of_solve_entail_wit_6 : solve_entail_wit_6.
+Axiom proof_of_solve_entail_wit_7 : solve_entail_wit_7.
+Axiom proof_of_solve_entail_wit_8 : solve_entail_wit_8.
+Axiom proof_of_solve_entail_wit_9 : solve_entail_wit_9.
+Axiom proof_of_solve_entail_wit_10 : solve_entail_wit_10.
+Axiom proof_of_solve_return_wit_1 : solve_return_wit_1.
+Axiom proof_of_solve_return_wit_2 : solve_return_wit_2.
+Axiom proof_of_solve_partial_solve_wit_1_pure : solve_partial_solve_wit_1_pure.
+Axiom proof_of_solve_partial_solve_wit_1 : solve_partial_solve_wit_1.
+Axiom proof_of_solve_partial_solve_wit_2_pure : solve_partial_solve_wit_2_pure.
+Axiom proof_of_solve_partial_solve_wit_2 : solve_partial_solve_wit_2.
+Axiom proof_of_solve_partial_solve_wit_3 : solve_partial_solve_wit_3.
+Axiom proof_of_solve_partial_solve_wit_4 : solve_partial_solve_wit_4.
+Axiom proof_of_solve_partial_solve_wit_5 : solve_partial_solve_wit_5.
+Axiom proof_of_solve_partial_solve_wit_6 : solve_partial_solve_wit_6.
+Axiom proof_of_solve_partial_solve_wit_7 : solve_partial_solve_wit_7.
+Axiom proof_of_solve_partial_solve_wit_8 : solve_partial_solve_wit_8.
+Axiom proof_of_solve_partial_solve_wit_9_pure : solve_partial_solve_wit_9_pure.
+Axiom proof_of_solve_partial_solve_wit_9 : solve_partial_solve_wit_9.
+Axiom proof_of_solve_partial_solve_wit_10 : solve_partial_solve_wit_10.
+Axiom proof_of_solve_partial_solve_wit_11 : solve_partial_solve_wit_11.
+Axiom proof_of_solve_partial_solve_wit_12_pure : solve_partial_solve_wit_12_pure.
+Axiom proof_of_solve_partial_solve_wit_12 : solve_partial_solve_wit_12.
+
+End VC_Correct.
