QCP_examples/humaneval/spec_logic_rewrite_c_files/C_161_proof_manual.v
@@ -1,0 +1,338 @@
+Require Import Coq.ZArith.ZArith.
+Require Import Coq.Bool.Bool.
+Require Import Coq.Strings.String.
+Require Import Coq.Strings.Ascii.
+Require Import Coq.Lists.List.
+Require Import Coq.Classes.RelationClasses.
+Require Import Coq.Classes.Morphisms.
+Require Import Coq.micromega.Psatz.
+Require Import Coq.Sorting.Permutation.
+From AUXLib Require Import int_auto Axioms Feq Idents ListLib VMap.
+Require Import SetsClass.SetsClass. Import SetsNotation.
+From SimpleC.SL Require Import Mem SeparationLogic.
+From SimpleC.EE Require Import C_161_goal.
+From SimpleC.EE Require Import C_161_proof_auto.
+Require Import Logic.LogicGenerator.demo932.Interface.
+Local Open Scope Z_scope.
+Local Open Scope sets.
+Local Open Scope string_scope.
+Local Open Scope list.
+Import naive_C_Rules.
+Require Import SimpleC.StdLib.string_lib.
+Require Import coins_161.
+Local Open Scope sac.
+
+Lemma proof_of_solve_entail_wit_1_split_goal_1 : solve_entail_wit_1_split_goal_1.
+Proof.
+  unfold solve_entail_wit_1_split_goal_1.
+  intros. entailer!.
+  apply flip_scan_state_z_161_init.
+Qed.
+
+Lemma proof_of_solve_entail_wit_1_split_goal_2 : solve_entail_wit_1_split_goal_2.
+Proof.
+  unfold solve_entail_wit_1_split_goal_2.
+  intros. entailer!.
+  rewrite PreH3. apply string_length_nonneg.
+Qed.
+
+Lemma proof_of_solve_entail_wit_1_split_goal_spatial : solve_entail_wit_1_split_goal_spatial.
+Proof. unfold solve_entail_wit_1_split_goal_spatial. intros. entailer!. Qed.
+
+Lemma proof_of_solve_entail_wit_1 : solve_entail_wit_1.
+Proof.
+  unfold solve_entail_wit_1.
+  right. intros. entailer!.
+  - rewrite PreH3. apply string_length_nonneg.
+  - apply flip_scan_state_z_161_init.
+Qed.
+
+Lemma proof_of_solve_entail_wit_2_1_split_goal_1 : solve_entail_wit_2_1_split_goal_1.
+Proof.
+  unfold solve_entail_wit_2_1_split_goal_1.
+  intros. entailer!.
+  assert (Hi : 0 <= i < Zlength input).
+  { unfold string_length in PreH7. lia. }
+  assert (Hc : 0 <= Znth i (c_string input) 0 <= 127).
+  { apply c_string_char_bound; [exact PreH16 |]. unfold string_length. lia. }
+  rewrite signed_last_nbits_8_eq_161 by exact Hc.
+  rewrite c_string_inside_eq_161 by exact Hi.
+  eapply flip_scan_state_z_161_step_nonletter; try eassumption.
+  - reflexivity.
+  - unfold upper_z_161. rewrite <- c_string_inside_eq_161 by exact Hi. lia.
+  - unfold lower_z_161. rewrite <- c_string_inside_eq_161 by exact Hi. lia.
+Qed.
+
+Lemma proof_of_solve_entail_wit_2_1_split_goal_2 : solve_entail_wit_2_1_split_goal_2.
+Proof.
+  unfold solve_entail_wit_2_1_split_goal_2.
+  intros. entailer!.
+  pose proof (c_string_char_bound input i PreH16) as Hc.
+  specialize (Hc ltac:(unfold string_length in PreH7 |- *; lia)). lia.
+Qed.
+
+Lemma proof_of_solve_entail_wit_2_1 : solve_entail_wit_2_1.
+Proof.
+  unfold solve_entail_wit_2_1. right. intros. entailer!.
+  - pose proof (c_string_char_bound input i PreH16) as Hc.
+    specialize (Hc ltac:(unfold string_length in PreH7 |- *; lia)). lia.
+  - assert (Hi : 0 <= i < Zlength input).
+    { unfold string_length in PreH7. lia. }
+    assert (Hc : 0 <= Znth i (c_string input) 0 <= 127).
+    { apply c_string_char_bound; [exact PreH16 |]. unfold string_length. lia. }
+    rewrite signed_last_nbits_8_eq_161 by exact Hc.
+    rewrite c_string_inside_eq_161 by exact Hi.
+    eapply flip_scan_state_z_161_step_nonletter; try eassumption.
+    + reflexivity.
+    + unfold upper_z_161. rewrite <- c_string_inside_eq_161 by exact Hi. lia.
+    + unfold lower_z_161. rewrite <- c_string_inside_eq_161 by exact Hi. lia.
+Qed.
+
+Lemma proof_of_solve_entail_wit_2_2_split_goal_1 : solve_entail_wit_2_2_split_goal_1.
+Proof.
+  unfold solve_entail_wit_2_2_split_goal_1.
+  intros. entailer!.
+  assert (Hi : 0 <= i < Zlength input).
+  { unfold string_length in PreH5. lia. }
+  assert (Hc : 0 <= Znth i (c_string input) 0 <= 127).
+  { apply c_string_char_bound; [exact PreH14 |]. unfold string_length. lia. }
+  rewrite signed_last_nbits_8_eq_161 by exact Hc.
+  rewrite c_string_inside_eq_161 by exact Hi.
+  eapply flip_scan_state_z_161_step_nonletter; try eassumption.
+  - reflexivity.
+  - unfold upper_z_161. rewrite <- c_string_inside_eq_161 by exact Hi. lia.
+  - unfold lower_z_161. rewrite <- c_string_inside_eq_161 by exact Hi. lia.
+Qed.
+
+Lemma proof_of_solve_entail_wit_2_2_split_goal_2 : solve_entail_wit_2_2_split_goal_2.
+Proof.
+  unfold solve_entail_wit_2_2_split_goal_2.
+  intros. entailer!.
+  pose proof (c_string_char_bound input i PreH14) as Hc.
+  specialize (Hc ltac:(unfold string_length in PreH5 |- *; lia)). lia.
+Qed.
+
+Lemma proof_of_solve_entail_wit_2_2 : solve_entail_wit_2_2.
+Proof.
+  unfold solve_entail_wit_2_2. right. intros. entailer!.
+  - pose proof (c_string_char_bound input i PreH14) as Hc.
+    specialize (Hc ltac:(unfold string_length in PreH5 |- *; lia)). lia.
+  - assert (Hi : 0 <= i < Zlength input).
+    { unfold string_length in PreH5. lia. }
+    assert (Hc : 0 <= Znth i (c_string input) 0 <= 127).
+    { apply c_string_char_bound; [exact PreH14 |]. unfold string_length. lia. }
+    rewrite signed_last_nbits_8_eq_161 by exact Hc.
+    rewrite c_string_inside_eq_161 by exact Hi.
+    eapply flip_scan_state_z_161_step_nonletter; try eassumption.
+    + reflexivity.
+    + unfold upper_z_161. rewrite <- c_string_inside_eq_161 by exact Hi. lia.
+    + unfold lower_z_161. rewrite <- c_string_inside_eq_161 by exact Hi. lia.
+Qed.
+
+Lemma proof_of_solve_entail_wit_2_3_split_goal_1 : solve_entail_wit_2_3_split_goal_1.
+Proof.
+  unfold solve_entail_wit_2_3_split_goal_1.
+  intros. entailer!.
+  assert (Hi : 0 <= i < Zlength input).
+  { unfold string_length in PreH6. lia. }
+  rewrite c_string_inside_eq_161 by exact Hi.
+  eapply flip_scan_state_z_161_step_nonletter; try eassumption.
+  - reflexivity.
+  - unfold upper_z_161. rewrite <- c_string_inside_eq_161 by exact Hi. lia.
+  - unfold lower_z_161. rewrite <- c_string_inside_eq_161 by exact Hi. lia.
+Qed.
+
+Lemma proof_of_solve_entail_wit_2_3 : solve_entail_wit_2_3.
+Proof.
+  unfold solve_entail_wit_2_3. right. intros. entailer!.
+  assert (Hi : 0 <= i < Zlength input).
+  { unfold string_length in PreH6. lia. }
+  rewrite c_string_inside_eq_161 by exact Hi.
+  eapply flip_scan_state_z_161_step_nonletter; try eassumption.
+  - reflexivity.
+  - unfold upper_z_161. rewrite <- c_string_inside_eq_161 by exact Hi. lia.
+  - unfold lower_z_161. rewrite <- c_string_inside_eq_161 by exact Hi. lia.
+Qed.
+
+Lemma proof_of_solve_entail_wit_2_4_split_goal_1 : solve_entail_wit_2_4_split_goal_1.
+Proof.
+  unfold solve_entail_wit_2_4_split_goal_1.
+  intros. entailer!.
+  assert (Hi : 0 <= i < Zlength input).
+  { unfold string_length in PreH7. lia. }
+  rewrite c_string_inside_eq_161 by exact Hi.
+  eapply flip_scan_state_z_161_step_lower; try eassumption.
+  - reflexivity.
+  - unfold upper_z_161. rewrite <- c_string_inside_eq_161 by exact Hi. lia.
+  - unfold lower_z_161. rewrite <- c_string_inside_eq_161 by exact Hi. lia.
+Qed.
+
+Lemma proof_of_solve_entail_wit_2_4 : solve_entail_wit_2_4.
+Proof.
+  unfold solve_entail_wit_2_4. right. intros. entailer!.
+  assert (Hi : 0 <= i < Zlength input).
+  { unfold string_length in PreH7. lia. }
+  rewrite c_string_inside_eq_161 by exact Hi.
+  eapply flip_scan_state_z_161_step_lower; try eassumption.
+  - reflexivity.
+  - unfold upper_z_161. rewrite <- c_string_inside_eq_161 by exact Hi. lia.
+  - unfold lower_z_161. rewrite <- c_string_inside_eq_161 by exact Hi. lia.
+Qed.
+
+Lemma proof_of_solve_entail_wit_2_5_split_goal_1 : solve_entail_wit_2_5_split_goal_1.
+Proof.
+  unfold solve_entail_wit_2_5_split_goal_1.
+  intros. entailer!.
+  assert (Hi : 0 <= i < Zlength input).
+  { unfold string_length in PreH5. lia. }
+  rewrite c_string_inside_eq_161 by exact Hi.
+  eapply flip_scan_state_z_161_step_upper; try eassumption.
+  - reflexivity.
+  - unfold upper_z_161. rewrite <- c_string_inside_eq_161 by exact Hi. lia.
+Qed.
+
+Lemma proof_of_solve_entail_wit_2_5 : solve_entail_wit_2_5.
+Proof.
+  unfold solve_entail_wit_2_5. right. intros. entailer!.
+  assert (Hi : 0 <= i < Zlength input).
+  { unfold string_length in PreH5. lia. }
+  rewrite c_string_inside_eq_161 by exact Hi.
+  eapply flip_scan_state_z_161_step_upper; try eassumption.
+  - reflexivity.
+  - unfold upper_z_161. rewrite <- c_string_inside_eq_161 by exact Hi. lia.
+Qed.
+
+Lemma proof_of_solve_entail_wit_4 : solve_entail_wit_4.
+Proof.
+  unfold solve_entail_wit_4. right. intros.
+  assert (i = n) by lia. subst i.
+  Exists output_2. entailer!.
+Qed.
+
+Lemma proof_of_solve_entail_wit_5 : solve_entail_wit_5.
+Proof.
+  unfold solve_entail_wit_5. right. intros.
+  subst nletter.
+  destruct (flip_scan_state_z_161_finish_no_letter
+    input output_2 n PreH4 PreH9) as [Hnone Hflip].
+  assert (Hflipout : flip_output_z_161 input output_2).
+  { exact Hflip. }
+  assert (Hvalidout : valid_string output_2).
+  { rewrite Hflip. apply flip_output_valid_161. exact PreH10. }
+  Exists output_2. unfold c_string. entailer!.
+Qed.
+
+Lemma proof_of_solve_entail_wit_6 : solve_entail_wit_6.
+Proof.
+  unfold solve_entail_wit_6. right. intros.
+  Exists output_2. entailer!.
+  apply reverse_scan_state_z_161_init.
+  rewrite PreH5. apply string_length_nonneg.
+Qed.
+
+Lemma proof_of_solve_entail_wit_7 : solve_entail_wit_7.
+Proof.
+  unfold solve_entail_wit_7. right. intros.
+  Exists output_2. entailer!.
+  assert (Hj : 0 <= j < Zlength input).
+  { unfold string_length in PreH4. lia. }
+  assert (Hk : 0 <= (n - 1) - j < Zlength input).
+  { unfold string_length in PreH4. lia. }
+  rewrite c_string_inside_eq_161 by exact Hk.
+  eapply reverse_scan_state_z_161_step; try eassumption.
+  unfold string_length in PreH4. rewrite PreH4. reflexivity.
+Qed.
+
+Lemma proof_of_solve_entail_wit_9 : solve_entail_wit_9.
+Proof.
+  unfold solve_entail_wit_9. right. intros.
+  assert (j = n) by lia. subst j.
+  assert (Hnlen : n = Zlength input).
+  { unfold string_length in PreH3. exact PreH3. }
+  pose proof (reverse_scan_state_z_161_finish
+    input rev_output_2 n Hnlen PreH12) as Hrev.
+  assert (Hrevout : reverse_output_z_161 input rev_output_2).
+  { exact Hrev. }
+  assert (Hvalidrev : valid_string rev_output_2).
+  { rewrite Hrev. apply rev_valid_161. exact PreH13. }
+  assert (Hspec : problem_161_spec_z input rev_output_2).
+  { eapply problem_161_spec_z_intro_rev; eauto. }
+  Exists rev_output_2 output_2. entailer!.
+Qed.
+
+Lemma proof_of_solve_entail_wit_10 : solve_entail_wit_10.
+Proof.
+  unfold solve_entail_wit_10. right. intros.
+  assert (Hnlen : n = Zlength input).
+  { unfold string_length in PreH4. exact PreH4. }
+  destruct (flip_scan_state_z_161_finish_has_letter
+    input output_2 n nletter Hnlen PreH1 PreH9) as [Hhas Hflip].
+  assert (Hflipout : flip_output_z_161 input output_2).
+  { exact Hflip. }
+  assert (Hvalidout : valid_string output_2).
+  { rewrite Hflip. apply flip_output_valid_161. exact PreH10. }
+  assert (Hspec : problem_161_spec_z input output_2).
+  { eapply problem_161_spec_z_intro_flip; eauto. }
+  Exists output_2. unfold c_string. entailer!.
+Qed.
+
+Lemma proof_of_solve_return_wit_1 : solve_return_wit_1.
+Proof.
+  unfold solve_return_wit_1. right. intros.
+  Exists output_2. unfold string_length.
+  rewrite (flip_output_z_161_length input output_2 PreH8).
+  unfold string_length in PreH3. entailer!.
+  rewrite <- PreH3. entailer!.
+Qed.
+
+Lemma proof_of_solve_return_wit_2 : solve_return_wit_2.
+Proof.
+  unfold solve_return_wit_2. right. intros.
+  Exists rev_output. unfold string_length.
+  rewrite (reverse_output_z_161_length input rev_output PreH12).
+  unfold string_length in PreH4. entailer!.
+  rewrite <- PreH4. entailer!.
+Qed.
+
+Lemma proof_of_solve_partial_solve_wit_2_pure_split_goal_1 : solve_partial_solve_wit_2_pure_split_goal_1.
+Proof.
+  unfold solve_partial_solve_wit_2_pure_split_goal_1.
+  intros. entailer!.
+  rewrite PreH5. pose proof (string_length_nonneg input). lia.
+Qed.
+
+Lemma proof_of_solve_partial_solve_wit_2_pure : solve_partial_solve_wit_2_pure.
+Proof.
+  unfold solve_partial_solve_wit_2_pure. right. intros. entailer!.
+  rewrite PreH5. pose proof (string_length_nonneg input). lia.
+Qed.
+
+Lemma proof_of_solve_partial_solve_wit_9_pure_split_goal_1 : solve_partial_solve_wit_9_pure_split_goal_1.
+Proof.
+  unfold solve_partial_solve_wit_9_pure_split_goal_1.
+  intros. entailer!.
+  rewrite PreH11. pose proof (string_length_nonneg input). lia.
+Qed.
+
+Lemma proof_of_solve_partial_solve_wit_9_pure : solve_partial_solve_wit_9_pure.
+Proof.
+  unfold solve_partial_solve_wit_9_pure. right. intros. entailer!.
+  rewrite PreH11. pose proof (string_length_nonneg input). lia.
+Qed.
+
+Lemma proof_of_solve_partial_solve_wit_12_pure_split_goal_1 : solve_partial_solve_wit_12_pure_split_goal_1.
+Proof.
+  unfold solve_partial_solve_wit_12_pure_split_goal_1.
+  intros. entailer!.
+  rewrite Zlength_c_string_161.
+  rewrite (flip_output_z_161_length input output PreH21).
+  unfold string_length in PreH14. lia.
+Qed.
+
+Lemma proof_of_solve_partial_solve_wit_12_pure : solve_partial_solve_wit_12_pure.
+Proof.
+  unfold solve_partial_solve_wit_12_pure. right. intros. entailer!.
+  rewrite Zlength_c_string_161.
+  rewrite (flip_output_z_161_length input output PreH21).
+  unfold string_length in PreH14. lia.
+Qed.
